proof/invariant-abstract/DetSchedSchedule_AI.thy
@@ -2145,7 +2145,7 @@ crunches sched_context_donate
 abbreviation cur_sc_offset_sufficient :: "time \<Rightarrow> 'z state \<Rightarrow> bool"
 where
   "cur_sc_offset_sufficient usage s \<equiv>
-      is_refill_sufficient usage (cur_sc s) s"
+      cur_sc s \<noteq> idle_sc_ptr \<longrightarrow> is_refill_sufficient usage (cur_sc s) s"
 
 abbreviation cur_sc_budget_sufficient :: "'z state \<Rightarrow> bool"
 where
@@ -2240,6 +2240,7 @@ definition cur_sc_more_than_ready_2 where
   "cur_sc_more_than_ready_2 cons_time c_time rf_cfgs csc \<equiv>
      cons_time \<noteq> 0
      \<longrightarrow> pred_map active_scrc rf_cfgs csc
+     \<longrightarrow> csc \<noteq> idle_sc_ptr
      \<longrightarrow> pred_map (refill_ready_no_overflow_sc cons_time c_time) rf_cfgs csc
           \<and> pred_map (refill_sufficient_sc cons_time) rf_cfgs csc"
 
@@ -4743,7 +4744,7 @@ lemma charge_budget_is_active_sc[wp]:
   "charge_budget consumed canTimeout \<lbrace>\<lambda>s :: 'state_ext state. P (is_active_sc sc_ptr s)\<rbrace>"
   apply (clarsimp simp: charge_budget_def refill_reset_rr_def update_refill_tl_def
                         update_sched_context_set_refills_rewrite update_refill_hd_def)
-  apply (wpsimp wp: hoare_drop_imps set_refills_wp get_refills_wp)
+  apply (wpsimp wp: hoare_drop_imps set_refills_wp get_refills_wp is_round_robin_wp)
   apply (clarsimp simp: vs_all_heap_simps active_sc_def obj_at_kh_kheap_simps pred_map_simps)
   done
 
@@ -9798,7 +9799,8 @@ lemma handle_overrun_loop_head_bound:
         \<and> pred_map (\<lambda>cfg. refills_unat_sum (scrc_refills cfg) = unat (scrc_budget cfg))
                    (sc_refill_cfgs_of s) (cur_sc s)
         \<and> pred_map (\<lambda>cfg. scrc_budget cfg \<le> scrc_period cfg) (sc_refill_cfgs_of s) (cur_sc s)
-        \<and> pred_map (\<lambda>cfg. MIN_REFILLS \<le> scrc_refill_max cfg) (sc_refill_cfgs_of s) (cur_sc s)\<rbrace>
+        \<and> pred_map (\<lambda>cfg. MIN_REFILLS \<le> scrc_refill_max cfg) (sc_refill_cfgs_of s) (cur_sc s)
+        \<and> cur_sc s \<noteq> idle_sc_ptr\<rbrace>
    handle_overrun_loop usage
    \<lbrace>\<lambda>_ s. pred_map (\<lambda>cfg. unat (r_time (hd (scrc_refills cfg))) + 4 * unat MAX_PERIOD \<le> unat max_time)
                    (sc_refill_cfgs_of s) (cur_sc s)\<rbrace>"
@@ -10464,7 +10466,8 @@ lemma refill_budget_check_non_zero_refills_helper:
   done
 
 lemma refill_budget_check_valid_refills[wp]:
-  "\<lbrace>\<lambda>s. valid_refills sc_ptr s \<and> cur_sc_offset_ready 0 s \<and> current_time_bounded 5 s\<rbrace>
+  "\<lbrace>\<lambda>s. valid_refills sc_ptr s \<and> cur_sc_offset_ready 0 s \<and> current_time_bounded 5 s
+        \<and> cur_sc s \<noteq> idle_sc_ptr\<rbrace>
    refill_budget_check usage
    \<lbrace>\<lambda>_ s. valid_refills sc_ptr s\<rbrace>"
   supply map_map[simp del] round_robin_def[simp add]
@@ -10505,6 +10508,7 @@ lemma refill_budget_check_valid_refills[wp]:
                                                   \<le> unat max_time)
                                            (sc_refill_cfgs_of s) (cur_sc s)
                                 \<and> cur_sc s = sc_ptr
+                                \<and> cur_sc s \<noteq> idle_sc_ptr
                                 \<and> (pred_map (\<lambda>cfg. r_time (hd (scrc_refills cfg)) < MAX_RELEASE_TIME)
                                             (sc_refill_cfgs_of s) sc_ptr
                                    \<longrightarrow> pred_map (\<lambda>cfg. usage' < r_amount (hd (scrc_refills cfg)))
@@ -10545,7 +10549,7 @@ lemma refill_budget_check_valid_refills[wp]:
                            \<and> pred_map (\<lambda>cfg. refills_unat_sum (scrc_refills cfg)
                                               = unat (scrc_budget cfg))
                                        (sc_refill_cfgs_of s) sc_ptr
-                           \<and> sc_ptr = cur_sc s"
+                           \<and> sc_ptr = cur_sc s \<and> cur_sc s \<noteq> idle_sc_ptr"
                in hoare_seq_ext[rotated])
    apply (rule hoare_when_cases, clarsimp simp: vs_all_heap_simps)
    apply (rule hoare_seq_ext[OF _ get_sched_context_sp])
@@ -10581,7 +10585,7 @@ lemma refill_budget_check_valid_refills[wp]:
    apply (wpsimp wp: refill_budget_check_refills_unat_sum_helper, fastforce+)
   apply (clarsimp simp: obj_at_def)
   apply (wpsimp wp: set_refills_wp get_refills_wp
-              simp: vs_all_heap_simps update_sched_context_set_refills_rewrite update_refill_hd_rewrite)
+              simp: vs_all_heap_simps update_sched_context_set_refills_rewrite update_refill_hd_rewrite)+
   done
 
 lemma valid_refills_sc_update:
@@ -11096,7 +11100,7 @@ method handle_overrun_loop_fail_simple
 
 lemma refill_budget_check_refill_ready_offset_ready_and_sufficient:
   "\<lbrace>\<lambda>s. if sc_ptr = cur_sc s
-        then valid_refills (cur_sc s) s \<and> current_time_bounded 5 s
+        then valid_refills (cur_sc s) s \<and> current_time_bounded 5 s \<and> cur_sc s \<noteq> idle_sc_ptr
              \<and> cur_sc_offset_ready usage s \<and> cur_sc_offset_sufficient usage s
         else is_refill_ready sc_ptr s\<rbrace>
    refill_budget_check usage
@@ -11148,7 +11152,7 @@ lemma refill_budget_check_refill_ready_offset_ready_and_sufficient:
                             \<and> pred_map (\<lambda>cfg. refills_unat_sum (scrc_refills cfg)
                                               = unat (scrc_budget cfg))
                                        (sc_refill_cfgs_of s) (cur_sc s)
-                            \<and> csc_ptr = cur_sc s
+                            \<and> csc_ptr = cur_sc s \<and> cur_sc s \<noteq> idle_sc_ptr
                             \<and> (pred_map (\<lambda>cfg. r_time (hd (scrc_refills cfg)) < MAX_RELEASE_TIME)
                                          (sc_refill_cfgs_of s) (cur_sc s)
                                \<longrightarrow> pred_map (\<lambda>cfg. rv < r_amount (hd (scrc_refills cfg)))
@@ -11213,7 +11217,7 @@ lemma is_refill_sufficient_0_alt:
 
 lemma refill_budget_check_is_refill_sufficient:
   "\<lbrace>\<lambda>s. if sc_ptr = cur_sc s
-        then valid_refills (cur_sc s) s \<and> current_time_bounded 0 s
+        then valid_refills (cur_sc s) s \<and> current_time_bounded 0 s \<and> cur_sc s \<noteq> idle_sc_ptr
              \<and> cur_sc_offset_ready usage s \<and> cur_sc_offset_sufficient usage s
          else is_refill_sufficient 0 sc_ptr s\<rbrace>
    refill_budget_check usage
@@ -11251,7 +11255,7 @@ lemma refill_budget_check_is_refill_sufficient:
                                            = unat (scrc_budget cfg))
                                     (sc_refill_cfgs_of s) (cur_sc s)
                                 \<and> valid_refills (cur_sc s) s
-                                \<and> csc_ptr = cur_sc s
+                                \<and> csc_ptr = cur_sc s \<and> cur_sc s \<noteq> idle_sc_ptr
                                 \<and> \<not> round_robin (cur_sc s) s
                                 \<and> (pred_map (\<lambda>cfg. r_time (hd (scrc_refills cfg)) < MAX_RELEASE_TIME)
                                              (sc_refill_cfgs_of s) (cur_sc s)
@@ -11293,7 +11297,7 @@ crunches refill_budget_check
 
 lemma refill_budget_check_round_robin_refill_ready_offset_ready_and_sufficient:
   "\<lbrace>\<lambda>s. if sc_ptr = cur_sc s
-        then current_time_bounded 0 s
+        then current_time_bounded 0 s \<and> cur_sc s \<noteq> idle_sc_ptr
              \<and> cur_sc_offset_ready usage s \<and> cur_sc_offset_sufficient usage s
          else is_refill_ready sc_ptr s\<rbrace>
    refill_budget_check_round_robin usage
@@ -11307,7 +11311,7 @@ lemma refill_budget_check_round_robin_refill_ready_offset_ready_and_sufficient:
 
 lemma refill_budget_check_round_robin_is_refill_sufficient:
   "\<lbrace>\<lambda>s. if sc_ptr = cur_sc s
-        then valid_refills (cur_sc s) s \<and> current_time_bounded 0 s
+        then valid_refills (cur_sc s) s \<and> current_time_bounded 0 s \<and> cur_sc s \<noteq> idle_sc_ptr
              \<and> cur_sc_offset_ready usage s \<and> cur_sc_offset_sufficient usage s
          else is_refill_sufficient 0 sc_ptr s\<rbrace>
    refill_budget_check_round_robin usage
@@ -11475,6 +11479,7 @@ lemma refill_budget_check_round_robin_active_sc_tcb_at[wp]:
 lemma refill_budget_check_valid_ready_qs_offset_ready_and_sufficient:
   "\<lbrace>\<lambda>s. valid_ready_qs s \<and> cur_sc_active s \<and> current_time_bounded 1 s
         \<and> active_sc_valid_refills s
+        \<and> cur_sc s \<noteq> idle_sc_ptr
         \<and> cur_sc_offset_ready usage s \<and> cur_sc_offset_sufficient usage s
         \<and> current_time_bounded 5 s\<rbrace>
    refill_budget_check usage
@@ -11493,7 +11498,7 @@ lemma refill_budget_check_valid_ready_qs_offset_ready_and_sufficient:
 
 lemma refill_budget_check_valid_ready_qs:
   "\<lbrace>\<lambda>s. valid_ready_qs s \<and> cur_sc_active s
-        \<and> active_sc_valid_refills s
+        \<and> active_sc_valid_refills s \<and> cur_sc s \<noteq> idle_sc_ptr
         \<and> ((cur_sc_offset_ready usage s \<and> cur_sc_offset_sufficient usage s )
             \<or> (sc_not_in_ready_q (cur_sc s) s))
         \<and> current_time_bounded 5 s\<rbrace>
@@ -11504,14 +11509,16 @@ lemma refill_budget_check_valid_ready_qs:
   apply (rule refill_budget_check_valid_ready_qs_offset_ready_and_sufficient)
   apply (rule refill_budget_check_valid_ready_qs_not_queued)
   apply (strengthen current_time_bounded_strengthen[where k=5])
-  by simp
+  apply fastforce
+  done
 
 lemma refill_budget_check_round_robin_valid_ready_qs_offset_ready_and_sufficient:
   "\<lbrace>\<lambda>s. valid_ready_qs s
         \<and> active_sc_valid_refills s
         \<and> pred_map (\<lambda>cfg. scrc_period cfg = 0) (sc_refill_cfgs_of s) (cur_sc s)
         \<and> cur_sc_offset_ready usage s \<and> cur_sc_offset_sufficient usage s
-        \<and> current_time_bounded 2 s \<and> unat usage + unat MAX_PERIOD \<le> unat max_time\<rbrace>
+        \<and> current_time_bounded 2 s \<and> unat usage + unat MAX_PERIOD \<le> unat max_time
+        \<and> cur_sc s \<noteq> idle_sc_ptr\<rbrace>
    refill_budget_check_round_robin usage
    \<lbrace>\<lambda>_. valid_ready_qs\<rbrace>"
   apply (rule hoare_lift_Pf2[where f="ready_queues", rotated], wpsimp)
@@ -11532,7 +11539,8 @@ lemma refill_budget_check_round_robin_valid_ready_qs:
          current_time_bounded 2 s \<and> pred_map (\<lambda>cfg. scrc_period cfg = 0) (sc_refill_cfgs_of s) (cur_sc s) \<and>
          unat usage + unat MAX_PERIOD \<le> unat max_time \<and>
         ((cur_sc_offset_ready usage s \<and> cur_sc_offset_sufficient usage s )
-         \<or> (sc_not_in_ready_q (cur_sc s) s))\<rbrace>
+         \<or> (sc_not_in_ready_q (cur_sc s) s))
+        \<and> cur_sc s \<noteq> idle_sc_ptr\<rbrace>
    refill_budget_check_round_robin usage
    \<lbrace>\<lambda>_. valid_ready_qs\<rbrace>"
   apply (rule_tac Q="\<lambda>_ s. valid_ready_qs s \<or> valid_ready_qs s" in hoare_strengthen_post[rotated], simp)
@@ -11557,7 +11565,7 @@ lemma commit_time_valid_release_q:
   unfolding commit_time_def
   apply (rule hoare_seq_ext[OF _ gets_sp])
   apply (rule hoare_seq_ext[OF _ get_sched_context_sp])
-  apply (case_tac "sc_active sc"; simp add: bind_assoc)
+  apply (case_tac "sc_active sc \<and> csc \<noteq> idle_sc_ptr"; simp add: bind_assoc)
    apply (rule hoare_seq_ext[OF _ gets_sp])
    apply (rename_tac csc sc consumed)
   apply (rule_tac P="\<lambda>s. \<exists>tp. bound_sc_tcb_at ((=) (Some (cur_sc s))) tp s" in hoare_pre_tautI)
@@ -11638,7 +11646,8 @@ lemma commit_time_released_ipc_queues[wp]:
   apply (rule hoare_weaken_pre)
    apply (rule_tac R="cur_sc_more_than_ready and current_time_bounded 5
                       and (\<lambda>s. consumed = consumed_time s) and cur_sc_active
-                      and (\<lambda>s. valid_refills (cur_sc s) s)"
+                      and (\<lambda>s. valid_refills (cur_sc s) s)
+                      and (\<lambda>s. csc = cur_sc s)"
           in released_ipc_queues_lift_pre_conj)
     apply (wpsimp simp: budget_ready_def2
                     wp: hoare_vcg_ex_lift
@@ -11743,10 +11752,9 @@ lemma refill_budget_check_schedule_used_r_time_helper:
   apply (subst unat_sub | subst unat_add_lem'' | linarith
          | clarsimp simp: word_le_nat_alt word_less_nat_alt no_overflow_def unat_sub window_def)+
   done
-
 lemma refill_budget_check_bounded_release_time:
   "\<lbrace>bounded_release_time sc_ptr and cur_sc_offset_ready 0 and current_time_bounded 5
-    and valid_refills sc_ptr\<rbrace>
+    and valid_refills sc_ptr and (\<lambda>s. cur_sc s \<noteq> idle_sc_ptr)\<rbrace>
    refill_budget_check usage
    \<lbrace>\<lambda>_. bounded_release_time sc_ptr\<rbrace>"
   (is "valid _ _ ?post")
@@ -11787,7 +11795,7 @@ lemma refill_budget_check_bounded_release_time:
                                                    + 4 * unat MAX_PERIOD
                                                    \<le> unat max_time)
                                             (sc_refill_cfgs_of s) (cur_sc s)
-                                \<and> cur_sc s = sc_ptr
+                                \<and> cur_sc s = sc_ptr \<and> cur_sc s \<noteq> idle_sc_ptr
                                 \<and> (pred_map (\<lambda>cfg. r_time (hd (scrc_refills cfg)) < MAX_RELEASE_TIME)
                                              (sc_refill_cfgs_of s) sc_ptr
                                    \<longrightarrow> pred_map (\<lambda>cfg. usage' < r_amount (hd (scrc_refills cfg)))
@@ -11826,7 +11834,7 @@ lemma refill_budget_check_bounded_release_time:
                            \<and> pred_map (\<lambda>cfg. refills_unat_sum (scrc_refills cfg)
                                               = unat (scrc_budget cfg))
                                        (sc_refill_cfgs_of s) sc_ptr
-                           \<and> sc_ptr = cur_sc s
+                           \<and> sc_ptr = cur_sc s \<and> cur_sc s \<noteq> idle_sc_ptr
                            \<and> pred_map (\<lambda>cfg. unat (r_time (scrc_refill_hd cfg)) + 3 * unat MAX_PERIOD
                                              \<le> unat max_time)
                                       (sc_refill_cfgs_of s) (cur_sc s)"
@@ -11835,14 +11843,16 @@ lemma refill_budget_check_bounded_release_time:
     apply ( clarsimp simp: vs_all_heap_simps current_time_bounded_def)
    apply (rule hoare_seq_ext[OF _ get_sched_context_sp])
    apply (intro hoare_vcg_conj_lift_pre_fix; (solves schedule_used_simple)?)
-           apply (wpsimp wp: refill_budget_check_refills_sum_helper)
-          apply (wpsimp wp: refill_budget_check_ordered_disjoint_helper', fastforce+)
-         apply (wpsimp wp: refill_budget_check_no_overflow', fastforce+)
-        apply (wpsimp wp: refill_budget_check_window_helper, fastforce+)
-       apply (wpsimp wp: refill_budget_check_length_helper)
-      apply (wpsimp wp: refill_budget_check_non_zero_refills_helper)
-     apply (wpsimp wp: refill_budget_check_refills_unat_sum_helper, fastforce+)
-    apply wpsimp
+            apply (wpsimp wp: refill_budget_check_refills_sum_helper)
+           apply (wpsimp wp: refill_budget_check_ordered_disjoint_helper', fastforce+)
+          apply (wpsimp wp: refill_budget_check_no_overflow', fastforce+)
+         apply (wpsimp wp: refill_budget_check_window_helper, fastforce+)
+        apply (wpsimp wp: refill_budget_check_length_helper)
+       apply (wpsimp wp: refill_budget_check_non_zero_refills_helper)
+      apply (wpsimp wp: refill_budget_check_refills_unat_sum_helper, fastforce+)
+     apply wpsimp
+    apply (wpsimp wp: set_refills_wp get_refills_wp
+                simp: vs_all_heap_simps update_sched_context_set_refills_rewrite update_refill_hd_rewrite)
    apply (wpsimp wp: refill_budget_check_schedule_used_r_time_helper, fastforce+)
   apply (rule_tac Q="\<lambda>_ s. pred_map (\<lambda>cfg. unat (r_time (scrc_refill_hd cfg)) + 2 * unat MAX_PERIOD
                                            \<le> unat max_time) (sc_refill_cfgs_of s) sc_ptr"
@@ -11859,7 +11869,7 @@ lemma refill_budget_check_round_robin_active_sc_valid_refills:
     and (\<lambda>s. pred_map (\<lambda>cfg. scrc_period cfg = 0) (sc_refill_cfgs_of s) (cur_sc s))
     and K (unat consumed + unat MAX_PERIOD \<le> unat max_time)
     and cur_sc_offset_sufficient consumed
-    and current_time_bounded 1\<rbrace>
+    and current_time_bounded 1 and (\<lambda>s. cur_sc s \<noteq> idle_sc_ptr)\<rbrace>
    refill_budget_check_round_robin consumed
    \<lbrace>\<lambda>_. active_sc_valid_refills\<rbrace>"
   unfolding active_sc_valid_refills_def
@@ -11875,7 +11885,7 @@ lemma cur_sc_bounded_release_helper:
 lemma refill_budget_check_active_sc_valid_refills:
   "\<lbrace>active_sc_valid_refills
     and cur_sc_offset_ready 0
-    and current_time_bounded 5\<rbrace>
+    and current_time_bounded 5 and (\<lambda>s. cur_sc s \<noteq> idle_sc_ptr)\<rbrace>
    refill_budget_check consumed
    \<lbrace>\<lambda>_. active_sc_valid_refills\<rbrace>"
   unfolding active_sc_valid_refills_def
@@ -12049,7 +12059,8 @@ lemma refill_unblock_check_cur_sc_more_than_ready[wp]:
    \<lbrace>\<lambda>_. cur_sc_more_than_ready\<rbrace>"
   apply (wpsimp wp: hoare_vcg_imp_lift' simp: cur_sc_more_than_ready_def)
     apply (wps, wpsimp)
-   apply (wps, wpsimp wp: refill_unblock_check_refill_ready_no_overflow_sc ruc_is_refill_sufficient_indep)
+   apply (wps, wpsimp wp: refill_unblock_check_refill_ready_no_overflow_sc
+                          ruc_is_refill_sufficient_indep hoare_vcg_imp_lift')
   apply clarsimp
   done
 
@@ -12057,11 +12068,7 @@ lemma if_cond_refill_unblock_check_cur_sc_more_than_ready[wp]:
   "\<lbrace>cur_sc_more_than_ready and (\<lambda>s. \<forall>scp. scopt = Some scp \<longrightarrow> scp \<noteq> cur_sc s)\<rbrace>
    if_cond_refill_unblock_check scopt act ast
    \<lbrace>\<lambda>_. cur_sc_more_than_ready\<rbrace>"
-  apply (wpsimp wp: hoare_vcg_imp_lift' simp: cur_sc_more_than_ready_def)
-   apply (wps, wpsimp wp: refill_unblock_check_refill_ready_no_overflow_sc ruc_is_refill_sufficient_indep
-                    simp: if_cond_refill_unblock_check_def)+
-  apply clarsimp
-  done
+  by (wpsimp simp: if_cond_refill_unblock_check_def)
 
 lemma cur_tcb_sc_at:
   "\<lbrakk>valid_objs s; cur_tcb s; bound_sc_tcb_at ((=) (Some sc_ptr)) (cur_thread s) s\<rbrakk>
@@ -17592,7 +17599,7 @@ lemma charge_budget_valid_blocked[wp]:
   unfolding charge_budget_def refill_reset_rr_def update_refill_hd_def
             update_refill_tl_def update_sched_context_set_refills_rewrite
   by (wpsimp wp: reschedule_required_valid_blocked end_timeslice_valid_blocked
-                 assert_inv gts_wp is_schedulable_wp')
+                 assert_inv gts_wp is_schedulable_wp' is_round_robin_wp)
 
 lemma refill_reset_rr_valid_release_q[wp]:
   "\<lbrace>valid_release_q and sc_refills_sc_at (\<lambda>refills. length refills = 2) scp\<rbrace>
@@ -17632,11 +17639,11 @@ lemma charge_budget_valid_release_q:
                        split: if_splits)
        apply (wpsimp wp: sc_consumed_add_invs)
       apply (wpsimp wp: refill_budget_check_valid_release_q is_round_robin_wp)+
-  apply (intro conjI impI allI)
    apply (clarsimp simp: valid_refills_def vs_all_heap_simps rr_valid_refills_def
-                         sc_at_pred_n_def obj_at_def
+                         sc_at_pred_n_def obj_at_def ct_in_state_def pred_tcb_at_def
+                         runnable_eq_active
                   split: if_splits)
-  apply (fastforce simp: cur_sc_chargeable_def pred_map_simps obj_at_def valid_release_q_def
+  apply (fastforce simp: cur_sc_chargeable_def obj_at_def valid_release_q_def
                          in_queue_2_def vs_all_heap_simps)
   done
 
@@ -17679,17 +17686,17 @@ lemma charge_budget_valid_sched_action:
           apply (rule_tac hoare_strengthen_post[rotated], erule ct_active_sc_helper)
           apply (wpsimp wp: hoare_vcg_all_lift hoare_vcg_imp_lift')
          apply (wpsimp wp: hoare_vcg_disj_lift hoare_vcg_imp_lift')
-         apply (wpsimp wp: hoare_vcg_all_lift hoare_vcg_imp_lift')
-       apply wpsimp
+         apply (wpsimp wp: hoare_vcg_all_lift hoare_vcg_imp_lift')+
       apply (wpsimp wp: refill_reset_rr_valid_sched_action
-                        refill_budget_check_valid_sched_action_act_not)
+                        refill_budget_check_valid_sched_action_act_not)+
      apply (wpsimp wp: is_round_robin_wp)+
-  apply (clarsimp simp: valid_sched_def valid_sched_action_def)
+  apply (clarsimp simp: valid_sched_def valid_sched_action_def split: if_splits)
   apply (subgoal_tac "sc_scheduler_act_not (cur_sc s) s", simp)
   apply (intro conjI impI allI)
   apply (clarsimp simp: cur_sc_chargeable_def scheduler_act_sane_def)
-  apply (subgoal_tac "pred_map runnable (tcb_sts_of s) t")
-  apply (drule_tac x=t in spec)+
+  apply (rename_tac t')
+  apply (subgoal_tac "pred_map runnable (tcb_sts_of s) t'")
+  apply (drule_tac x=t' in spec)+
   apply (fastforce simp: pred_map_simps)
   apply (clarsimp simp:  weak_valid_sched_action_def in_queue_2_def)
   done
@@ -17778,12 +17785,15 @@ lemma charge_budget_released_ipc_queues:
   supply if_split [split del]
   apply (clarsimp simp: charge_budget_def)
   apply (wpsimp wp: end_timeslice_released_ipc_queues assert_inv gts_wp is_schedulable_wp')
-       apply (rule_tac Q="\<lambda>_. released_ipc_queues and active_sc_valid_refills" in hoare_strengthen_post[rotated]
+       apply (rule_tac Q="\<lambda>_. released_ipc_queues and active_sc_valid_refills
+                              and (\<lambda>s. cur_sc s \<noteq> idle_sc_ptr)"
+                    in hoare_strengthen_post[rotated]
               , clarsimp simp: tcb_at_kh_simps ct_in_state_def runnable_eq_active split: if_splits)
        apply (wpsimp wp: refill_budget_check_released_ipc_queues
                          refill_budget_check_active_sc_valid_refills
                          is_round_robin_wp' get_sched_context_wp gets_wp)+
-  by (clarsimp simp: vs_all_heap_simps active_sc_valid_refills_def)
+  apply (clarsimp simp: vs_all_heap_simps active_sc_valid_refills_def split: if_splits)
+  done
 
 lemma ct_not_blocked_cur_sc_not_blocked:
   "cur_sc_chargeable s \<Longrightarrow> ct_not_blocked s \<Longrightarrow> cur_sc_not_blocked s"
@@ -17830,22 +17840,22 @@ lemma charge_budget_valid_ready_qs:
                         refill_budget_check_released_ipc_queues
                         refill_budget_check_valid_sched_action_act_not)
      apply (wpsimp wp: is_round_robin_wp)+
+  apply (clarsimp split: if_splits)
   apply (subgoal_tac "sc_not_in_ready_q (cur_sc s) s \<and> sc_scheduler_act_not (cur_sc s) s", simp)
-  apply (intro conjI impI allI)
-      apply (clarsimp simp: active_sc_valid_refills_def)
-     apply (clarsimp simp: vs_all_heap_simps pred_map_def obj_at_def)
-    apply (clarsimp simp: active_sc_valid_refills_def)
-   apply (clarsimp simp: vs_all_heap_simps pred_map_def obj_at_def)
+   apply (fastforce simp: vs_all_heap_simps pred_map_def obj_at_def ct_in_state_def pred_tcb_at_def
+                          active_sc_valid_refills_def cur_sc_chargeable_def runnable_eq_active)
+  apply (clarsimp simp: vs_all_heap_simps pred_map_def obj_at_def ct_in_state_def pred_tcb_at_def)
   apply (intro conjI impI allI)
    apply (clarsimp simp: cur_sc_chargeable_def)
    apply (subgoal_tac "pred_map runnable (tcb_sts_of s) t")
     apply (drule_tac x=t in spec)+
-    apply (clarsimp simp: pred_map_simps, fastforce)
+    apply (fastforce simp: vs_all_heap_simps valid_ready_qs_def in_queue_2_def runnable_eq_active
+                    split: thread_state.splits)
    apply (clarsimp simp: valid_ready_qs_def in_queue_2_def in_ready_q_def)
   apply (clarsimp simp: cur_sc_chargeable_def scheduler_act_sane_def)
   apply (subgoal_tac "pred_map runnable (tcb_sts_of s) t")
    apply (drule_tac x=t in spec)+
-   apply (fastforce simp: pred_map_simps)
+   apply (clarsimp simp: vs_all_heap_simps valid_ready_qs_def in_queue_2_def in_ready_q_def)
   apply (clarsimp simp: valid_sched_action_def weak_valid_sched_action_def)
   done
 
@@ -17888,8 +17898,11 @@ lemma charge_budget_active_reply_scs:
                     get_tcb_obj_ref_wp is_schedulable_wp)
       apply (rule_tac Q="\<lambda>_. active_reply_scs" in hoare_strengthen_post[rotated],
              clarsimp split: if_splits simp: schedulable_def2)
-  by (wpsimp simp: refill_reset_rr_def update_refill_hd_def update_sched_context_set_refills_rewrite
-                   update_refill_tl_def)+
+  apply (wpsimp simp: refill_reset_rr_def update_refill_hd_def update_sched_context_set_refills_rewrite
+                      update_refill_tl_def)+
+  apply (clarsimp simp: schedulable_def2
+                 split: if_splits)
+  done
 
 lemma charge_budget_ready_or_release:
   "\<lbrace>ready_or_release and ready_qs_etcb_eq and ct_not_in_release_q and ct_not_queued
@@ -17982,7 +17995,7 @@ lemma check_budget_active_sc_valid_refills:
   unfolding check_budget_def
   apply (wpsimp wp: charge_budget_active_sc_valid_refills)
   apply (intro conjI impI)
-   apply (fastforce elim: consumed_time_bounded_helper current_time_bounded_strengthen)
+   apply (clarsimp simp: current_time_bounded_def consumed_time_bounded_def)
   apply (clarsimp simp: refill_ready_no_overflow_def vs_all_heap_simps)
   done
 
@@ -18570,7 +18583,7 @@ lemma lookup_extra_caps_not_timeout[wp]:
   by (wpsimp wp: mapME_wp' lookup_cap_and_slot_valid_fault)
 
 lemma cur_sc_tcb_bound_ready:
-  "\<lbrakk>cur_sc_offset_ready k s; cur_sc_tcb_are_bound s; current_time_bounded l s\<rbrakk>
+  "\<lbrakk>cur_sc_offset_ready k s; cur_sc_tcb_are_bound s; current_time_bounded l s; cur_sc s \<noteq> idle_sc_ptr\<rbrakk>
    \<Longrightarrow> budget_ready (cur_thread s) s"
   apply (clarsimp simp: vs_all_heap_simps refill_ready_no_overflow_def refill_ready_def)
   apply (simp add: word_le_nat_alt unat_add_lem)
@@ -18578,11 +18591,11 @@ lemma cur_sc_tcb_bound_ready:
 
 lemma schact_is_rct_ct_released:
   "\<lbrakk>schact_is_rct s; cur_sc_active s; valid_sched s; invs s;
-    cur_sc_offset_ready k s; current_time_bounded j s\<rbrakk>
+    cur_sc_offset_ready k s; current_time_bounded j s; cur_sc s \<noteq> idle_sc_ptr\<rbrakk>
    \<Longrightarrow> ct_released s"
   apply (subgoal_tac "active_sc_tcb_at (cur_thread s) s")
   apply (clarsimp simp: released_sc_tcb_at_def)
-   apply (erule (1) cur_sc_tcb_bound_ready[OF _ invs_strengthen_cur_sc_tcb_are_bound], fastforce+)
+   apply (rule cur_sc_tcb_bound_ready[OF _ invs_strengthen_cur_sc_tcb_are_bound], fastforce+)
   apply (erule (2) cur_sc_active_ct_active_sc[OF _ invs_cur_sc_tcb_symref])
   done
 
@@ -18611,14 +18624,17 @@ lemma handle_invocation_valid_sched:
        apply (wp ct_in_state_set set_thread_state_runnable_valid_sched
                  sts_schedulable_scheduler_action
             hoare_vcg_E_conj | simp add: split_def if_apply_def2 split del: if_split)+
+  apply clarsimp
   apply (subgoal_tac "ct_released s")
    apply (clarsimp simp: valid_sched_def ct_not_in_q_def valid_ready_qs_def not_queued_def
                      schedulable_def2 ct_in_state_def runnable_eq_active not_in_release_q_def
                      in_release_queue_def released_sc_tcb_at_def)
    apply (fastforce elim: st_tcb_ex_cap st_tcb_at_strengthen_pred
-                          current_time_bounded_strengthen invs_retract_tcb_scps
+                          current_time_bounded_strengthen
                    intro: fault_tcbs_valid_states_active)
-  apply (fastforce intro: schact_is_rct_ct_released)
+  apply (rule schact_is_rct_ct_released; fastforce?)
+  apply (rule cur_sc_not_idle_sc_ptr; fastforce?)
+  apply (rule invs_strengthen_cur_sc_tcb_are_bound; fastforce)
   done
 
 end
@@ -18984,7 +19000,7 @@ lemma charge_budget_scheduler_act_sane[wp]:
    charge_budget consumed can_timeout
    \<lbrace>\<lambda>_. scheduler_act_sane ::'state_ext state \<Rightarrow> _\<rbrace>"
   unfolding charge_budget_def
-  by (wpsimp wp: is_schedulable_wp hoare_drop_imp)
+  by (wpsimp wp: is_schedulable_wp hoare_drop_imp is_round_robin_wp)
 
 lemma check_budget_scheduler_act_sane[wp]:
   "\<lbrace>scheduler_act_sane::'state_ext state \<Rightarrow> _\<rbrace>
@@ -20401,21 +20417,23 @@ method handle_event_valid_sched_single
                  intro: active_sc_valid_refillsE)
 
 method handle_event_valid_sched_combined
-  = ((wpsimp wp: handle_invocation_valid_sched handle_recv_valid_sched
+  = (wpsimp wp: handle_invocation_valid_sched handle_recv_valid_sched
                 check_budget_restart_valid_sched_weaker handle_invocation_current_time_bounded_5
           simp: schedulable_def2 active_sc_tcb_at_fold
-      | strengthen current_time_bounded_strengthen[where n=2 and k=5, simplified])+
-     , simp add: imp_conjR
-     , ((wpsimp wp: hoare_vcg_conj_lift
-         | wpsimp wp: check_budget_restart_true check_budget_restart_valid_sched_weaker
-                     update_time_stamp_current_time_bounded_5 hoare_drop_imps)+
-     , subgoal_tac "ct_released s"
-     , fastforce dest: valid_sched_ct_not_queued
-                 elim: active_from_running
-                 simp: runnable_eq_active released_sc_tcb_at_def
-                       active_sc_tcb_at_fold ct_in_state_def2[symmetric]
-                intro: active_sc_valid_refillsE)
-     , fastforce intro: schact_is_rct_ct_released)
+      | strengthen current_time_bounded_strengthen[where n=2 and k=5, simplified])+,
+    simp add: imp_conjR,
+    (wpsimp wp: hoare_vcg_conj_lift
+     | wpsimp wp: check_budget_restart_true check_budget_restart_valid_sched_weaker
+                  update_time_stamp_current_time_bounded_5 hoare_drop_imps)+,
+    subgoal_tac "ct_released s",
+    fastforce dest: valid_sched_ct_not_queued
+              elim: active_from_running
+              simp: runnable_eq_active released_sc_tcb_at_def
+                    active_sc_tcb_at_fold ct_in_state_def2[symmetric]
+             intro: active_sc_valid_refillsE,
+    (rule schact_is_rct_ct_released; fastforce?),
+    (frule invs_strengthen_cur_sc_tcb_are_bound; fastforce?),
+    (rule cur_sc_not_idle_sc_ptr; fastforce simp: ct_in_state_def pred_tcb_at_def obj_at_def)
 
 method handle_event_valid_sched_yield
   = (wpsimp wp: handle_yield_valid_sched
@@ -20436,9 +20454,15 @@ method handle_event_valid_sched_fault
      , clarsimp simp: valid_fault_def ct_in_state_def2[symmetric] is_timeout_fault_def
      , strengthen schact_is_rct_sane valid_sched_ct_not_queued
                   ct_runnable_ct_not_blocked
-     , simp
-     , (fastforce simp: ct_active_imp_not_timeout is_timeout_fault_def
-                 intro: active_sc_valid_refillsE schact_is_rct_ct_released)?)
+     , simp,subgoal_tac "ct_released s",
+    fastforce dest: valid_sched_ct_not_queued
+              elim: active_from_running
+              simp: runnable_eq_active released_sc_tcb_at_def
+                    active_sc_tcb_at_fold ct_in_state_def2[symmetric]
+             intro: active_sc_valid_refillsE,
+    (rule schact_is_rct_ct_released; fastforce?),
+    (frule invs_strengthen_cur_sc_tcb_are_bound; fastforce?),
+    (rule cur_sc_not_idle_sc_ptr; fastforce simp: ct_in_state_def pred_tcb_at_def obj_at_def))
 
 lemma handle_event_valid_sched:
   "\<lbrace>invs
@@ -20459,14 +20483,20 @@ lemma handle_event_valid_sched:
 
   (* SyscallEvent *)
        subgoal for syscall
-       by (case_tac syscall, simp_all add: handle_send_def handle_call_def liftE_bindE
-           , (handle_event_valid_sched_single
-              | handle_event_valid_sched_combined
-              | handle_event_valid_sched_yield)+) \<comment> \<open>takes 30 seconds or so\<close>
+         by (case_tac syscall, simp_all add: handle_send_def handle_call_def liftE_bindE
+             , (handle_event_valid_sched_single
+                | handle_event_valid_sched_combined
+                | handle_event_valid_sched_yield)+)
 
       apply (find_goal \<open>match premises in "_ = Interrupt" \<Rightarrow> \<open>-\<close>\<close>)
       defer
+
       apply handle_event_valid_sched_fault+
+
+   (* HypervisorEvent *)
+   apply wpsimp
+   apply (clarsimp simp: ct_in_state_def schact_is_rct_def valid_sched_def ct_not_in_q_def
+                         pred_tcb_at_def obj_at_def)
 
   (* Interrupt *)
   apply wpsimp
@@ -21531,7 +21561,8 @@ lemma charge_budget_ready_if_schedulable[wp]:
      apply (wpsimp wp: is_round_robin_wp)
     apply wpsimp
    apply wpsimp
-  by (clarsimp simp: vs_all_heap_simps obj_at_def)
+  apply (fastforce simp: vs_all_heap_simps obj_at_def cur_sc_chargeable_def split: if_splits)
+  done
 
 lemma check_budget_ct_ready_if_schedulable[wp]:
   "\<lbrace>ct_ready_if_schedulable and cur_sc_chargeable and active_sc_valid_refills
@@ -21542,22 +21573,11 @@ lemma check_budget_ct_ready_if_schedulable[wp]:
    check_budget
    \<lbrace>\<lambda>_. ct_ready_if_schedulable :: det_state \<Rightarrow> _\<rbrace>"
   unfolding check_budget_def
-  by wpsimp
+  apply wpsimp
+  apply (clarsimp simp: vs_all_heap_simps refill_ready_no_overflow_def)
+  done
 
 end
-
-lemma offset_ready_ct_ready_if_schedulable:
-  "(cur_sc_active s \<longrightarrow> cur_sc_offset_ready k s)
-   \<Longrightarrow> cur_sc_chargeable s
-   \<Longrightarrow> current_time_bounded 0 s
-   \<Longrightarrow> ct_ready_if_schedulable s"
-  unfolding ct_ready_if_schedulable_def
-  apply clarsimp
-  apply (frule (1) cur_sc_chargeable_when_ct_active_sc)
-  apply (clarsimp simp: vs_all_heap_simps tcb_at_kh_simps refill_ready_no_overflow_def refill_ready_def)
-  apply (simp add: word_le_nat_alt unat_add_lem)
-  apply (frule cur_time_no_overflow, simp add: unat_plus_simple)
-  done
 
 crunches handle_no_fault, reply_from_kernel
   for cur_sc_more_than_ready[wp]: cur_sc_more_than_ready
@@ -21762,6 +21782,20 @@ lemma cur_sc_active_offset_ready_and_sufficient_implies_cur_sc_more_than_ready:
   apply (clarsimp simp: cur_sc_more_than_ready_def)
   done
 
+lemma cur_sc_active_implies_cur_sc_offset_ready_rewrite:
+  "(cur_sc_active s \<longrightarrow> cur_sc_offset_ready (consumed_time s) s)
+   = (cur_sc s \<noteq> idle_sc_ptr
+      \<longrightarrow> cur_sc_active s
+      \<longrightarrow> pred_map (refill_ready_no_overflow_sc (consumed_time s) (cur_time s)) (sc_refill_cfgs_of s) (cur_sc s))"
+  by fastforce
+
+lemma cur_sc_active_implies_cur_sc_offset_sufficient_rewrite:
+  "(cur_sc_active s \<longrightarrow> cur_sc_offset_sufficient (consumed_time s) s)
+   = (cur_sc s \<noteq> idle_sc_ptr
+      \<longrightarrow> cur_sc_active s
+      \<longrightarrow> is_refill_sufficient (consumed_time s) (cur_sc s) s)"
+  by fastforce
+
 lemma reset_untyped_cap_cur_sc_active_implies_cur_sc_offset_ready[wp]:
   "\<lbrace>\<lambda>s. (cur_sc_active s \<longrightarrow> cur_sc_offset_ready (consumed_time s) s) \<and> valid_machine_time s\<rbrace>
    reset_untyped_cap slot
@@ -21772,8 +21806,40 @@ lemma reset_untyped_cap_cur_sc_active_implies_cur_sc_offset_ready[wp]:
   apply (rule hoare_seq_ext_skipE, wpsimp)
   apply clarsimp
   apply (intro conjI impI; (solves wpsimp)?)
+    apply (rule hoare_seq_ext_skipE)
+     apply (subst cur_sc_active_implies_cur_sc_offset_ready_rewrite)+
+     apply (rule hoare_validE_conj)
+      apply (rule valid_validE)
+      apply (rule hoare_weaken_pre)
+       apply (rule hoare_vcg_imp_lift')
+        apply wpsimp
+       apply wpsimp
+      apply fastforce
+     apply wpsimp
+    apply wpsimp
+   apply (rule hoare_seq_ext_skipE)
+    apply (subst cur_sc_active_implies_cur_sc_offset_ready_rewrite)+
+    apply (rule hoare_validE_conj)
+     apply (rule valid_validE)
+     apply (rule hoare_weaken_pre)
+      apply (rule hoare_vcg_imp_lift')
+       apply wpsimp
+      apply wpsimp
+     apply fastforce
+    apply wpsimp
+   apply wpsimp
+  apply (rule hoare_seq_ext_skipE)
+   apply (subst cur_sc_active_implies_cur_sc_offset_ready_rewrite)+
+   apply (rule hoare_validE_conj)
+    apply (rule valid_validE)
+    apply (rule hoare_weaken_pre)
+     apply (rule hoare_vcg_imp_lift')
+      apply wpsimp
+     apply wpsimp
+    apply fastforce
+   apply wpsimp
+  apply wpsimp
   apply (rule_tac Q="?pre" in hoare_weaken_preE[rotated], simp)
-  apply (rule hoare_seq_ext_skipE, wpsimp)
   apply (rule valid_validE)
   apply (rule hoare_strengthen_post)
    apply (rule mapME_x_wp_inv)
@@ -21787,16 +21853,25 @@ lemma reset_untyped_cap_cur_sc_active_implies_cur_sc_offset_sufficient[wp]:
    reset_untyped_cap slot
    \<lbrace>\<lambda>_ s :: det_state. cur_sc_active s \<longrightarrow> cur_sc_offset_sufficient (consumed_time s) s\<rbrace>, -"
   (is "\<lbrace>?pre\<rbrace> _ \<lbrace>_\<rbrace>, -")
+  supply if_split[split del]
   apply (clarsimp simp: reset_untyped_cap_def)
   apply (clarsimp simp: validE_R_def)
-  apply (rule hoare_seq_ext_skipE, wpsimp)
+  apply (rule hoare_seq_ext_skipE)
+   apply wpsimp
+  apply (split if_splits)
+  apply (intro conjI)
+   apply wpsimp
   apply clarsimp
-  apply (intro conjI impI; (solves wpsimp)?)
-  apply (rule_tac Q="?pre" in hoare_weaken_preE[rotated], simp)
-  apply (rule hoare_seq_ext_skipE, wpsimp)
-  apply (rule_tac Q="\<lambda>_ . ?pre" and E="\<top>\<top>"in hoare_post_impErr; simp)
-  apply (rule mapME_x_wp_inv')
-  apply wpsimp
+  apply (rule_tac B="\<lambda>_ s. cur_sc_active s \<longrightarrow> cur_sc_offset_sufficient (consumed_time s) s"
+              and E="\<top>\<top>"
+               in hoare_vcg_seqE[rotated])
+   apply (subst cur_sc_active_implies_cur_sc_offset_sufficient_rewrite)+
+   apply (rule hoare_weaken_preE)
+    apply (rule hoare_vcg_imp_liftE)
+     apply wpsimp
+    apply wpsimp
+   apply fastforce
+  apply (wpsimp wp: mapME_x_wp_inv')
   done
 
 lemma invoke_untyped_cur_sc_active_implies_cur_sc_offset_ready[wp]:
@@ -21807,7 +21882,21 @@ lemma invoke_untyped_cur_sc_active_implies_cur_sc_offset_ready[wp]:
   apply (cases iv; simp)
   apply (clarsimp simp: validE_R_def whenE_def)
   apply (intro conjI impI)
+   apply (rule validE_valid)
+   apply (rule hoare_seq_ext_skipE, wpsimp)
+   apply (rule valid_validE)
+   apply (subst cur_sc_active_implies_cur_sc_offset_ready_rewrite)+
    apply (wpsimp wp: mapM_x_wp_inv)+
+      apply (rule hoare_vcg_imp_lift')
+       apply wpsimp
+      apply wpsimp
+     apply wpsimp
+    apply wpsimp
+   apply fastforce
+  apply (subst cur_sc_active_implies_cur_sc_offset_ready_rewrite)+
+  apply (wpsimp wp: mapM_x_wp_inv)+
+     apply (rule hoare_vcg_imp_lift')
+      apply wpsimp+
   done
 
 lemma invoke_untyped_cur_sc_active_implies_cur_sc_offset_sufficient[wp]:
@@ -21818,7 +21907,23 @@ lemma invoke_untyped_cur_sc_active_implies_cur_sc_offset_sufficient[wp]:
   apply (cases iv; simp)
   apply (clarsimp simp: validE_R_def whenE_def)
   apply (intro conjI impI)
-   apply (wpsimp wp: mapM_x_wp_inv)+
+  apply (rule hoare_seq_ext_skipE, wpsimp)
+   apply (wpsimp wp: mapM_x_wp_inv)
+      apply (subst cur_sc_active_implies_cur_sc_offset_sufficient_rewrite)+
+       apply (rule hoare_vcg_imp_lift')
+       apply wpsimp
+      apply wpsimp
+     apply wpsimp
+    apply wpsimp
+   apply fastforce
+  apply (subst cur_sc_active_implies_cur_sc_offset_sufficient_rewrite)+
+  apply (wpsimp wp: mapM_x_wp_inv)+
+     apply (rule hoare_vcg_imp_lift')
+      apply wpsimp
+     apply wpsimp
+    apply wpsimp
+   apply wpsimp
+  apply fastforce
   done
 
 lemma invoke_untyped_cur_sc_more_than_ready[wp]:
@@ -22242,7 +22347,8 @@ lemma check_budget_restart_true':
    handle_invocation calling blocking can_donate first_phase cptr
    \<lbrace>\<lambda>_. cur_sc_more_than_ready :: det_state \<Rightarrow> _\<rbrace>, -"
   unfolding handle_invocation_def
-  apply (wpsimp wp: syscall_valid hoare_drop_imp simp: cap_cap_slot_fold sc_at_kh_simps)
+  apply (wpsimp wp: syscall_valid simp: cap_cap_slot_fold sc_at_kh_simps
+         | wp (once) hoare_drop_imps)+
   apply (clarsimp simp: cur_sc_more_than_ready_def cong: conj_cong)
   apply (fastforce dest: sym_ref_tcb_sc invs_sym_refs invs_strengthen_cur_sc_tcb_are_bound
                    simp: vs_all_heap_simps)
@@ -22405,7 +22511,7 @@ lemma heap_refs_inv_sc_tcb:
                       heap_refs_retract_def)
 
 lemma sched_context_resume_cur_sc_not_in_release_q:
-  "\<lbrace>\<lambda>s. sc_not_in_release_q (cur_sc s) s
+  "\<lbrace>\<lambda>s. sc_not_in_release_q (cur_sc s) s \<and> sc_ptr \<noteq> idle_sc_ptr
         \<and> (if sc_ptr = cur_sc s
            then (cur_sc_active s \<longrightarrow> is_refill_ready (cur_sc s) s
                                      \<and> is_refill_sufficient 0 (cur_sc s) s)
@@ -22426,7 +22532,7 @@ lemma sched_context_resume_cur_sc_not_in_release_q:
   done
 
 lemma sched_context_resume_cur_sc_in_release_q_imp_zero_consumed:
-  "\<lbrace>\<lambda>s. cur_sc_in_release_q_imp_zero_consumed s
+  "\<lbrace>\<lambda>s. cur_sc_in_release_q_imp_zero_consumed s \<and> sc_ptr \<noteq> idle_sc_ptr
         \<and> (if sc_ptr = cur_sc s
            then (cur_sc_active s
                  \<longrightarrow> (consumed_time s \<noteq> 0
@@ -22469,11 +22575,50 @@ crunches refill_unblock_check, refill_update, refill_new
 
 context DetSchedSchedule_AI begin
 
+crunches tcb_sched_action, tcb_release_remove, reschedule_required
+  for ntfn_at_ppred[wp]: "\<lambda>s. ntfn_at_ppred proj P ntfn_ptr s"
+  (wp: crunch_wps)
+
+lemma sched_context_donate_ntfn_at_ppred[wp]:
+  "sched_context_donate a tcb_ptr \<lbrace>\<lambda>s. ntfn_at_ppred proj P ntfn_ptr s\<rbrace>"
+  apply (clarsimp simp: sched_context_donate_def test_reschedule_def)
+  apply (rule hoare_seq_ext_skip, wpsimp)
+  apply (rule hoare_seq_ext_skip)
+   apply (rule hoare_when_cases, simp)
+   apply (rule hoare_seq_ext_skip, wpsimp wp: update_sched_context_wp set_tcb_obj_ref_wp)+
+    apply (fastforce simp: ntfn_at_ppred_def obj_at_def)
+   apply (rule hoare_seq_ext_skip, wpsimp wp: update_sched_context_wp set_tcb_obj_ref_wp)+
+   apply wpsimp
+  apply (wpsimp wp: set_tcb_obj_ref_wp update_sched_context_wp)
+  apply (fastforce simp: ntfn_at_ppred_def obj_at_def)
+  done
+
+lemma ex_nonz_cap_to_ntfn_sc:
+  "\<lbrakk>ntfn_at_ppred ntfn_sc (\<lambda>f. f = Some sc_ptr) ntfn_ptr s; invs s;
+    sc_at sc_ptr s\<rbrakk>
+   \<Longrightarrow> ex_nonz_cap_to sc_ptr s"
+  apply (clarsimp simp: obj_at_def is_sc_obj_def)
+  apply (rule if_live_then_nonz_capD2)
+    apply fastforce
+   apply (clarsimp simp: obj_at_def is_sc_obj_def)
+   apply fastforce
+  apply (rename_tac ko n, case_tac ko; clarsimp)
+  apply (clarsimp simp: live_def live_sc_def ntfn_at_ppred_def obj_at_def)
+  apply (frule invs_sym_refs)
+  apply (prop_tac "(sc_ptr, NTFNSchedContext) \<in> state_refs_of s ntfn_ptr")
+   apply (clarsimp simp: state_refs_of_def)
+  apply (prop_tac "(ntfn_ptr, SCNtfn) \<in> state_refs_of s sc_ptr")
+   apply (clarsimp simp: sym_refs_def)
+   apply fastforce
+  apply (fastforce simp: state_refs_of_def)
+  done
+
 lemma maybe_donate_sc_cur_sc_not_in_release_q:
-  "\<lbrace>\<lambda>s. heap_refs_retract (sc_tcbs_of s) (tcb_scps_of s)
-        \<and> sc_not_in_release_q (cur_sc s) s
-        \<and> (cur_sc_active s \<longrightarrow> is_refill_ready (cur_sc s) s \<and> is_refill_sufficient 0 (cur_sc s) s)
-        \<and> not_in_release_q tcb_ptr s\<rbrace>
+  "\<lbrace>\<lambda>s. sc_not_in_release_q (cur_sc s) s
+        \<and> invs s
+        \<and> (cur_sc_active s \<and> cur_sc s \<noteq> idle_sc_ptr
+           \<longrightarrow> is_refill_ready (cur_sc s) s \<and> is_refill_sufficient 0 (cur_sc s) s)
+        \<and> not_in_release_q tcb_ptr s \<and> ex_nonz_cap_to tcb_ptr s\<rbrace>
    maybe_donate_sc tcb_ptr ntfn_ptr
    \<lbrace>\<lambda>_ s. sc_not_in_release_q (cur_sc s) s\<rbrace>"
   supply refill_unblock_check_cur_sc_budget_sufficient[wp del]
@@ -22487,15 +22632,35 @@ lemma maybe_donate_sc_cur_sc_not_in_release_q:
   apply (rule hoare_when_cases; (solves \<open>simp\<close>)?)
   apply (rule_tac B="\<lambda>_ s. heap_refs_retract (sc_tcbs_of s) (tcb_scps_of s)
                            \<and> sc_not_in_release_q (cur_sc s) s
-                           \<and> (cur_sc_active s \<longrightarrow> is_refill_ready (cur_sc s) s
-                                                  \<and> is_refill_sufficient 0 (cur_sc s) s)
-                           \<and> not_in_release_q tcb_ptr s"
+                           \<and> (cur_sc_active s \<and> cur_sc s  \<noteq> idle_sc_ptr
+                              \<longrightarrow> is_refill_ready (cur_sc s) s \<and> is_refill_sufficient 0 (cur_sc s) s)
+                           \<and> not_in_release_q tcb_ptr s
+                           \<and> ntfn_at_ppred ntfn_sc (\<lambda>f. f = Some a) ntfn_ptr s
+                           \<and> invs s
+                           \<and> ex_nonz_cap_to tcb_ptr s"
                in hoare_seq_ext[rotated])
-   apply ((wpsimp wp: sched_context_donate_sc_not_in_release_q sched_context_donate_sym_refs
-                      sched_context_donate_sym_refs
+   apply ((wpsimp wp: sched_context_donate_sc_not_in_release_q sched_context_donate_invs
            | wps)+)[1]
-   apply (clarsimp simp: vs_all_heap_simps obj_at_kh_kheap_simps)
-   apply (wpsimp wp: sched_context_resume_cur_sc_not_in_release_q)+
+   apply (clarsimp simp: vs_all_heap_simps obj_at_kh_kheap_simps is_tcb_def is_sc_obj_def)
+   apply (intro conjI impI)
+    apply (fastforce intro: ex_nonz_cap_to_ntfn_sc valid_objs_valid_sched_context_size
+                      simp: obj_at_def is_sc_obj_def)
+   apply (fastforce intro: valid_objs_valid_sched_context_size)
+  apply (wpsimp wp: sched_context_resume_cur_sc_not_in_release_q)+
+  apply (rename_tac ntfn_sc_ptr sc s)
+  apply (subgoal_tac "ntfn_sc_ptr \<noteq> idle_sc_ptr")
+   apply fastforce
+  apply (frule_tac scp=ntfn_sc_ptr in ex_nonz_cap_to_not_idle_sc_ptr)
+   apply (rule ex_nonz_cap_to_ntfn_sc)
+     apply fastforce
+    apply fastforce
+   apply (clarsimp simp: ntfn_at_ppred_def obj_at_def)
+   apply (rename_tac ntfn)
+   apply (prop_tac "valid_ntfn ntfn s")
+    apply (frule invs_valid_objs)
+    apply (fastforce simp: valid_objs_def valid_obj_def)
+   apply (clarsimp simp: valid_ntfn_def obj_at_def )
+  apply fastforce
   done
 
 end
@@ -22516,7 +22681,8 @@ lemma cur_sc_in_release_q_imp_zero_consumed_lift:
   by fast
 
 lemma cur_sc_more_than_ready_imp_cur_sc_ready_and_sufficient[elim]:
-  "\<lbrakk>cur_sc_more_than_ready s; consumed_time s \<noteq> 0; cur_sc_active s; current_time_bounded 0 s\<rbrakk>
+  "\<lbrakk>cur_sc_more_than_ready s; consumed_time s \<noteq> 0; cur_sc_active s; current_time_bounded 0 s;
+    cur_sc s \<noteq> idle_sc_ptr\<rbrakk>
    \<Longrightarrow> is_refill_ready (cur_sc s) s \<and> is_refill_sufficient 0 (cur_sc s) s"
   apply (clarsimp simp: cur_sc_more_than_ready_def is_refill_ready_def is_refill_sufficient_def
                         refill_ready_def vs_all_heap_simps refill_sufficient_def
@@ -22537,7 +22703,8 @@ lemma maybe_donate_sc_cur_sc_in_release_q_imp_zero_consumed:
   "\<lbrace>\<lambda>s. heap_refs_retract (sc_tcbs_of s) (tcb_scps_of s)
         \<and> cur_sc_in_release_q_imp_zero_consumed s
         \<and> cur_sc_more_than_ready s
-        \<and> not_in_release_q tcb_ptr s \<and> current_time_bounded 0 s\<rbrace>
+        \<and> not_in_release_q tcb_ptr s \<and> current_time_bounded 0 s \<and> ex_nonz_cap_to tcb_ptr s
+        \<and> invs s\<rbrace>
    maybe_donate_sc tcb_ptr ntfn_ptr
    \<lbrace>\<lambda>_. cur_sc_in_release_q_imp_zero_consumed\<rbrace>"
   unfolding cur_sc_in_release_q_imp_zero_consumed_def
@@ -22558,13 +22725,34 @@ lemma update_waiting_ntfn_cur_sc_in_release_q_imp_zero_consumed:
        \<and> cur_sc_in_release_q_imp_zero_consumed s
        \<and> cur_sc_more_than_ready s
        \<and> tcb_at (hd queue) s \<and> not_in_release_q (hd queue) s \<and> current_time_bounded 0 s
-       \<and> ex_nonz_cap_to ntfnptr s\<rbrace>
+       \<and> ex_nonz_cap_to ntfnptr s \<and> invs s\<rbrace>
    update_waiting_ntfn ntfnptr queue (ntfn_bound_tcb ntfn) (ntfn_sc ntfn) badge
    \<lbrace>\<lambda>_. cur_sc_in_release_q_imp_zero_consumed\<rbrace>"
+  supply if_split[split del] if_cong[cong]
   apply (clarsimp simp: update_waiting_ntfn_def)
-  by (wpsimp wp: set_thread_state_invs set_ntfn_minor_invs Arch.set_simple_ko_ioports
-                 maybe_donate_sc_cur_sc_in_release_q_imp_zero_consumed
-                 refill_unblock_check_active_sc_valid_refills maybeM_inv)
+  apply (wpsimp wp: set_thread_state_invs set_ntfn_minor_invs Arch.set_simple_ko_ioports
+                    maybe_donate_sc_cur_sc_in_release_q_imp_zero_consumed
+                    refill_unblock_check_active_sc_valid_refills maybeM_inv
+              simp: invs_def valid_state_def valid_pspace_def)
+  apply (prop_tac "valid_ntfn ntfn s")
+   apply (fastforce simp: valid_objs_def valid_obj_def obj_at_def)
+  apply (cases queue; clarsimp)
+  apply (intro conjI)
+       apply (clarsimp simp: pred_tcb_at_def obj_at_def)
+       apply (erule (1) if_live_then_nonz_capD2)
+       apply (fastforce simp: live_def
+                       split: thread_state.splits)
+      apply (clarsimp simp: valid_idle_def pred_tcb_at_def obj_at_def)
+     apply (clarsimp simp: replies_blocked_def pred_tcb_at_def obj_at_def)
+    apply (fastforce intro: update_waiting_notification_sym_refs_helper
+                      simp: obj_at_def valid_ntfn_def)
+   apply (clarsimp elim!: fault_tcbs_valid_states_not_fault_tcb_states
+                          pred_tcb_weakenE
+                    simp: pred_neg_def)
+   apply (case_tac "itcb_state tcb"; clarsimp)
+  apply (fastforce simp: valid_ntfn_def pred_tcb_at_def obj_at_def valid_bound_obj_def is_tcb_def
+                  split: list.splits option.splits)
+  done
 
 lemma cancel_ipc_heap_refs_retract_sc_tcbs_of[wp]:
   "cancel_ipc tptr \<lbrace>\<lambda>s. heap_refs_retract (sc_tcbs_of s) (tcb_scps_of s)\<rbrace>"
@@ -22615,12 +22803,16 @@ lemma send_signal_cur_sc_in_release_q_imp_zero_consumed:
   apply (rule hoare_seq_ext[OF _ gts_sp])
   apply (rule hoare_if; (solves \<open>wpsimp\<close>)?)
   apply (wpsimp wp: maybe_donate_sc_cur_sc_in_release_q_imp_zero_consumed
-                    sts_cancel_ipc_Running_invs cancel_ipc_invs_st_tcb_at)
-   apply (clarsimp simp: pred_tcb_at_def obj_at_def is_tcb_def)
-  apply (clarsimp simp: valid_sched_def valid_release_q_def in_release_q_def)
-  apply (drule_tac x=ntfn_tcb_ptr in bspec, simp)
-  apply (clarsimp simp: pred_tcb_at_def obj_at_def is_tcb_def vs_all_heap_simps receive_blocked_def)
-  apply (case_tac "tcb_state tcb"; clarsimp?)
+                    sts_cancel_ipc_Running_invs cancel_ipc_invs_st_tcb_at cancel_ipc_cap_to
+                    cancel_ipc_simple_except_awaiting_reply)
+  apply (clarsimp simp: pred_tcb_at_def obj_at_def is_tcb_def cong: conj_cong)
+  apply (intro conjI; fastforce?)
+   apply (erule valid_release_q_not_in_release_q_not_runnable)
+   apply (clarsimp simp: pred_tcb_at_def obj_at_def receive_blocked_def
+                  split: thread_state.splits)
+  apply (rule if_live_then_nonz_capD2; fastforce?)
+  apply (clarsimp simp: live_def)
+  apply (case_tac "tcb_state tcb"; clarsimp simp: receive_blocked_def)
   done
 
 lemma handle_interrupt_cur_sc_in_release_q_imp_zero_consumed:
@@ -22639,6 +22831,7 @@ lemma handle_interrupt_cur_sc_in_release_q_imp_zero_consumed:
   apply (clarsimp simp: cte_wp_at_def ex_nonz_cap_to_def)
   apply (case_tac cap; clarsimp?)
   by fastforce
+
 end
 
 lemma update_timestamp_cur_sc_in_release_q_imp_zero_consumed:
@@ -22936,7 +23129,7 @@ lemma reply_remove_cur_sc_in_release_q_imp_zero_consumed[wp]:
   by (clarsimp simp: in_release_q_def not_in_release_q_def)
 
 lemma strengthen_cur_sc_offset_ready:
-  "cur_sc_offset_ready (consumed_time s) s
+  "cur_sc_offset_ready (consumed_time s) s \<Longrightarrow> cur_sc s \<noteq> idle_sc_ptr
    \<Longrightarrow> (\<exists>k. current_time_bounded k s) \<Longrightarrow> is_refill_ready (cur_sc s) s"
   unfolding is_refill_ready_def cur_sc_offset_ready_def
   apply (clarsimp simp: sc_at_pred_n_def obj_at_def vs_all_heap_simps refill_ready_def)
@@ -22947,7 +23140,8 @@ lemma strengthen_cur_sc_offset_ready:
   done
 
 lemma strengthen_cur_sc_offset_sufficient:
-  "cur_sc_offset_sufficient (consumed_time s) s \<Longrightarrow> is_refill_sufficient 0 (cur_sc s) s"
+  "cur_sc_offset_sufficient (consumed_time s) s \<Longrightarrow> cur_sc s \<noteq> idle_sc_ptr
+   \<Longrightarrow> is_refill_sufficient 0 (cur_sc s) s"
   unfolding is_refill_ready_def cur_sc_offset_ready_def
   apply (clarsimp simp: sc_at_pred_n_def obj_at_def vs_all_heap_simps refill_ready_def)
   apply (clarsimp simp: refill_capacity_def refill_sufficient_def split: if_splits)
@@ -22960,7 +23154,8 @@ lemma do_reply_transfer_sc_not_in_release_q:
         \<and> heap_refs_inv (tcb_scps_of s) (sc_tcbs_of s)
         \<and> valid_release_q s \<and> active_sc_valid_refills s \<and> cur_sc_active s
         \<and> cur_sc_offset_ready (consumed_time s) s \<and> cur_sc_offset_sufficient (consumed_time s) s
-        \<and> current_time_bounded 2 s\<rbrace>
+        \<and> current_time_bounded 2 s
+        \<and> cur_sc s \<noteq> idle_sc_ptr\<rbrace>
    do_reply_transfer sender reply grant
    \<lbrace>\<lambda>_ s :: det_state. sc_not_in_release_q (cur_sc s) s\<rbrace>"
   apply (simp add: do_reply_transfer_def maybeM_def)
@@ -22979,7 +23174,7 @@ lemma do_reply_transfer_sc_not_in_release_q:
                            \<and> (cur_sc_active s \<longrightarrow> cur_sc_offset_ready (consumed_time s) s)
                            \<and> (cur_sc_active s \<longrightarrow> cur_sc_offset_sufficient (consumed_time s) s)
                            \<and> current_time_bounded 2 s
-                           \<and> not_in_release_q receiver s"
+                           \<and> not_in_release_q receiver s \<and> cur_sc s \<noteq> idle_sc_ptr"
            in hoare_seq_ext[rotated])
    apply (wpsimp wp: reply_remove_tcb_scps_of_retract reply_remove_valid_release_q
                      reply_remove_heap_refs_retract_sc_tcbs
@@ -23013,8 +23208,12 @@ lemma do_reply_transfer_sc_not_in_release_q:
    apply (clarsimp simp: vs_all_heap_simps receive_blocked_def) \<comment> \<open>kheap s receiver = Some (TCB y)\<close>
    apply (case_tac "tcb_state y"; clarsimp?)
   apply (wpsimp wp: postpone_cur_sc_not_in_release_q_other)
-  apply (frule strengthen_cur_sc_offset_sufficient, frule strengthen_cur_sc_offset_ready, fastforce)
-  apply (clarsimp simp: obj_at_def vs_all_heap_simps)
+  apply (frule strengthen_cur_sc_offset_sufficient[rotated])
+  apply fastforce
+  apply (frule strengthen_cur_sc_offset_ready[rotated], fastforce+)
+  apply (clarsimp simp: obj_at_def vs_all_heap_simps refill_ready_no_overflow_def
+                        refill_sufficient_def refill_ready_def refill_capacity_def
+                 split: if_splits)
   done
 
 lemma do_reply_transfer_consumed_time[wp]:
@@ -23051,7 +23250,8 @@ lemma do_reply_transfer_cur_sc_in_release_q_imp_zero_consumed:
         \<and> heap_refs_inv (tcb_scps_of s) (sc_tcbs_of s)
         \<and> valid_release_q s \<and> active_sc_valid_refills s \<and> cur_sc_active s
         \<and> cur_sc_offset_ready (consumed_time s) s \<and> cur_sc_offset_sufficient (consumed_time s) s
-        \<and> current_time_bounded 2 s\<rbrace>
+        \<and> current_time_bounded 2 s
+        \<and> cur_sc s \<noteq> idle_sc_ptr\<rbrace>
    do_reply_transfer sender reply grant
    \<lbrace>\<lambda>_ s :: det_state. cur_sc_in_release_q_imp_zero_consumed s\<rbrace>"
   unfolding cur_sc_in_release_q_imp_zero_consumed_def
@@ -23168,46 +23368,58 @@ lemma sched_context_zero_refill_max_active_sc_valid_refills[wp]:
 
 context DetSchedSchedule_AI_handle_hypervisor_fault_det_ext begin
 
+crunches refill_new, refill_update
+  for ct_in_state[wp]: "ct_in_state P"
+  (wp: crunch_wps)
+
 lemma invoke_sched_control_configure_flags_cur_sc_in_release_q_imp_zero_consumed[wp]:
   "\<lbrace>invs
     and valid_sched_control_inv iv
     and cur_sc_in_release_q_imp_zero_consumed
     and cur_sc_more_than_ready
     and current_time_bounded 0
-    and cur_sc_tcb_are_bound\<rbrace>
+    and cur_sc_tcb_are_bound and ct_active and cur_sc_tcb_are_bound\<rbrace>
    invoke_sched_control_configure_flags iv
    \<lbrace>\<lambda>_. cur_sc_in_release_q_imp_zero_consumed\<rbrace>"
   supply if_split[split del]
   apply (cases iv, simp)
   apply (rename_tac sc_ptr budget period mrefills badge flags)
   apply (simp add: invoke_sched_control_configure_flags_def)
-  apply (subst bind_assoc[symmetric])
   apply (rule_tac B="\<lambda>_ s. invs s
                            \<and> cur_sc_in_release_q_imp_zero_consumed s
                            \<and> cur_sc_more_than_ready s
                            \<and> current_time_bounded 0 s
                            \<and> ex_nonz_cap_to sc_ptr s
-                           \<and> sc_tcb_sc_at bound (cur_sc s) s"
-                 in hoare_seq_ext[rotated])
-   apply (wpsimp wp: update_sc_sporadic_invs')
-     apply (wpsimp wp: update_sched_context_wp)
+                           \<and> sc_tcb_sc_at bound (cur_sc s) s \<and> ex_nonz_cap_to sc_ptr s
+                           \<and> ct_active s \<and> cur_sc_tcb_are_bound s"
+               in hoare_seq_ext[rotated])
+   apply (intro hoare_vcg_conj_lift_pre_fix; (solves wpsimp)?)
     apply (wpsimp wp: update_sc_badge_invs')
-    apply (wpsimp wp: update_sched_context_wp)
-   apply clarsimp
-   apply (intro conjI impI allI)
-      apply (frule invs_valid_global_refs)
-      apply (frule invs_valid_objs)
-      using idle_sc_no_ex_cap apply blast
-     apply (clarsimp simp: sc_at_pred_n_def obj_at_def vs_all_heap_simps split: if_splits)
-     apply (drule invs_sym_refs)
-     using sym_ref_tcb_sc apply fastforce
-    apply (clarsimp simp: sc_at_pred_n_def obj_at_def)
+    apply (frule invs_valid_global_refs)
+    apply (frule invs_valid_objs)
+    using idle_sc_no_ex_cap apply blast
+   apply (wpsimp wp: update_sched_context_wp)
+   apply (clarsimp simp: sc_at_pred_n_def obj_at_def vs_all_heap_simps split: if_splits)
+   apply (drule invs_sym_refs)
+   apply (fastforce dest: sym_ref_tcb_sc)
+
+  apply (rule hoare_seq_ext_skip)
+   apply (intro hoare_vcg_conj_lift_pre_fix; (solves wpsimp)?)
+    apply (wpsimp wp: update_sc_sporadic_invs')
+    apply (frule invs_valid_global_refs)
+    apply (frule invs_valid_objs)
+    using idle_sc_no_ex_cap apply blast
+   apply (wpsimp wp: update_sched_context_wp)
+   apply (clarsimp simp: sc_at_pred_n_def obj_at_def vs_all_heap_simps split: if_splits)
+
   apply (rule hoare_seq_ext[OF _ get_sched_context_sp])
   apply (rule_tac B="\<lambda>_ s. cur_sc_in_release_q_imp_zero_consumed s
                            \<and> cur_sc_more_than_ready s
                            \<and> current_time_bounded 0 s
                            \<and> (cur_sc s = sc_ptr \<longrightarrow> consumed_time s = 0)
-                           \<and> heap_refs_retract (sc_tcbs_of s) (tcb_scps_of s)"
+                           \<and> heap_refs_retract (sc_tcbs_of s) (tcb_scps_of s)
+                           \<and> ex_nonz_cap_to sc_ptr s \<and> ct_active s \<and> invs s
+                           \<and> cur_sc_tcb_are_bound s"
          in hoare_seq_ext)
    apply wpsimp
        apply (wpsimp wp: sched_context_resume_cur_sc_in_release_q_imp_zero_consumed split: if_splits)
@@ -23216,11 +23428,24 @@ lemma invoke_sched_control_configure_flags_cur_sc_in_release_q_imp_zero_consumed
     apply (rule_tac Q="\<lambda>_ s. cur_sc_in_release_q_imp_zero_consumed s
                              \<and> cur_sc_more_than_ready s
                              \<and> heap_refs_retract (sc_tcbs_of s) (tcb_scps_of s)
-                             \<and> current_time_bounded 0 s"
+                             \<and> current_time_bounded 0 s \<and> ex_nonz_cap_to sc_ptr s
+                             \<and> ct_active s \<and> invs s \<and> cur_sc_tcb_are_bound s"
            in hoare_strengthen_post[rotated])
      apply (clarsimp simp: cur_sc_more_than_ready_def split: if_splits)
-     using strengthen_cur_sc_offset_ready strengthen_cur_sc_offset_sufficient apply blast
-    apply wpsimp
+     apply (intro conjI impI allI)
+        apply (rule cur_sc_not_idle_sc_ptr; fastforce)
+       apply (rule strengthen_cur_sc_offset_ready)
+         apply fastforce
+        apply (rule cur_sc_not_idle_sc_ptr; fastforce)
+       apply fastforce
+      apply (rule strengthen_cur_sc_offset_sufficient)
+       apply fastforce
+      apply (rule cur_sc_not_idle_sc_ptr; fastforce)
+     apply (rule ex_nonz_cap_to_not_idle_sc_ptr; fastforce)
+    apply (wpsimp wp: refill_update_invs)
+   apply simp
+   apply (prop_tac "sc_ptr \<noteq> idle_sc_ptr")
+    apply (rule ex_nonz_cap_to_not_idle_sc_ptr; fastforce)
    apply simp
   apply (wpsimp wp: hoare_vcg_imp_lift)
        apply (strengthen invs_retract_sc_tcbs)
@@ -23230,9 +23455,10 @@ lemma invoke_sched_control_configure_flags_cur_sc_in_release_q_imp_zero_consumed
      apply (rule_tac Q="\<lambda>_ s. cur_sc_in_release_q_imp_zero_consumed s
                               \<and> cur_sc_more_than_ready s
                               \<and> invs s
-                              \<and> current_time_bounded 0 s"
+                              \<and> current_time_bounded 0 s \<and> ct_active s \<and> cur_sc_tcb_are_bound s
+                              \<and> ex_nonz_cap_to sc_ptr s"
             in hoare_strengthen_post[rotated])
-      apply (fastforce split: if_split)
+      apply (clarsimp split: if_split)
      apply wpsimp
     apply (wpsimp wp: tcb_release_remove_cur_sc_in_release_q_imp_zero_consumed)
    apply wpsimp
@@ -23283,7 +23509,7 @@ lemma sched_context_bind_tcb_cur_sc_in_release_q_imp_zero_consumed_helper:
         \<and> cur_sc_in_release_q_imp_zero_consumed s
         \<and> (\<forall>t\<in>set (release_queue s). pred_map (not is_blocked_on_reply) (tcb_sts_of s) t)
         \<and> (\<forall>t\<in> set (release_queue s). pred_map (\<lambda>a. \<exists>y. a = Some y) (tcb_scps_of s) t)
-        \<and> current_time_bounded 0 s
+        \<and> current_time_bounded 0 s \<and> sc_ptr \<noteq> idle_sc_ptr
         \<and> (if sc_ptr = cur_sc s
            then cur_sc_more_than_ready s
            else heap_refs_inv (sc_tcbs_of s) (tcb_scps_of s))\<rbrace>
@@ -23291,7 +23517,7 @@ lemma sched_context_bind_tcb_cur_sc_in_release_q_imp_zero_consumed_helper:
       set_sc_obj_ref sc_tcb_update sc_ptr (Some tcb_ptr)
    od
    \<lbrace>\<lambda>_ s. cur_sc_in_release_q_imp_zero_consumed s
-          \<and> current_time_bounded 0 s
+          \<and> current_time_bounded 0 s \<and> sc_ptr \<noteq> idle_sc_ptr
           \<and> (if sc_ptr = cur_sc s
              then cur_sc_more_than_ready s
              else heap_refs_inv (sc_tcbs_of s) (tcb_scps_of s))\<rbrace>"
@@ -23314,8 +23540,12 @@ lemma sched_context_bind_tcb_cur_sc_in_release_q_imp_zero_consumed_helper:
    apply (rule hoare_vcg_conj_lift)
     apply (rule sched_context_bind_tcb_helper_cur_sc_in_release_q_imp_zero_consumed)
    apply (rule hoare_vcg_conj_lift, wpsimp)
+
+   apply (rule hoare_vcg_conj_lift)
+    apply wpsimp
    apply (clarsimp simp: heap_refs_inv_def)
    apply (rule hoare_vcg_conj_lift)
+
     apply (rule sched_context_bind_tcb_helper_heap_refs_retract_sc_tcbs)
    apply (rule sched_context_bind_tcb_helper_heap_refs_retract_tcb_scps)
   apply (clarsimp simp: heap_refs_inv_def)
@@ -23323,7 +23553,7 @@ lemma sched_context_bind_tcb_cur_sc_in_release_q_imp_zero_consumed_helper:
 
 lemma sched_context_resume_cur_sc_in_release_q_imp_zero_consumed_not_cur_sc:
   "\<lbrace>\<lambda>s. cur_sc_in_release_q_imp_zero_consumed s
-        \<and> sc_ptr \<noteq> cur_sc s \<and> heap_refs_retract (sc_tcbs_of s) (tcb_scps_of s)\<rbrace>
+        \<and> sc_ptr \<noteq> cur_sc s \<and> sc_ptr \<noteq> idle_sc_ptr \<and> heap_refs_retract (sc_tcbs_of s) (tcb_scps_of s)\<rbrace>
    sched_context_resume sc_ptr
    \<lbrace>\<lambda>_ s. cur_sc_in_release_q_imp_zero_consumed s\<rbrace>"
   apply (clarsimp simp: cur_sc_in_release_q_imp_zero_consumed_def)
@@ -23343,6 +23573,7 @@ lemma sched_context_bind_tcb_cur_sc_in_release_q_imp_zero_consumed[wp]:
         \<and> (\<forall>t\<in>set (release_queue s). pred_map (not is_blocked_on_reply) (tcb_sts_of s) t)
         \<and> (\<forall>t\<in> set (release_queue s). pred_map (\<lambda>a. \<exists>y. a = Some y) (tcb_scps_of s) t)
         \<and> current_time_bounded 0 s
+        \<and> sc_ptr \<noteq> idle_sc_ptr
         \<and> (if sc_ptr = cur_sc s
            then cur_sc_more_than_ready s
            else heap_refs_inv (sc_tcbs_of s) (tcb_scps_of s))\<rbrace>
@@ -23367,15 +23598,18 @@ lemma sched_context_bind_tcb_cur_sc_in_release_q_imp_zero_consumed[wp]:
   apply (rule_tac Q="(\<lambda>s. cur_sc_in_release_q_imp_zero_consumed s \<and> current_time_bounded 0 s
                       \<and> heap_refs_inv (sc_tcbs_of s) (tcb_scps_of s)
                       \<and> (\<exists>n. ko_at (SchedContext x n) sc_ptr s))
-                     and (\<lambda>s. cur_sc s = curscp) and K (sc_ptr \<noteq> curscp)"
+                     and (\<lambda>s. cur_sc s = curscp) and K (sc_ptr \<noteq> curscp)
+                     and K( sc_ptr \<noteq> idle_sc_ptr)"
          in hoare_weaken_pre[rotated])
    apply (clarsimp simp: pred_neg_def)
-  apply (wpsimp wp: sched_context_resume_cur_sc_in_release_q_imp_zero_consumed_not_cur_sc)  apply (clarsimp simp: heap_refs_inv_def split: if_splits)
+  apply (wpsimp wp: sched_context_resume_cur_sc_in_release_q_imp_zero_consumed_not_cur_sc)
+  apply (clarsimp simp: heap_refs_inv_def split: if_splits)
   done
 
 lemma sched_context_yield_to_cur_sc_in_release_q_imp_zero_consumed[wp]:
   "\<lbrace>\<lambda>s. cur_sc_in_release_q_imp_zero_consumed s
         \<and> current_time_bounded 0 s
+        \<and> sc_ptr \<noteq> idle_sc_ptr
         \<and> (if sc_ptr = cur_sc s
            then cur_sc_more_than_ready s
            else heap_refs_inv (sc_tcbs_of s) (tcb_scps_of s))\<rbrace>
@@ -23423,52 +23657,108 @@ lemma invoke_sched_context_cur_sc_in_release_q_imp_zero_consumed[wp]:
    invoke_sched_context i
    \<lbrace>\<lambda>rv. cur_sc_in_release_q_imp_zero_consumed\<rbrace>"
   apply (cases i; wpsimp simp: invoke_sched_context_def sched_context_unbind_all_tcbs_def)
-  apply (fastforce simp: obj_at_kh_kheap_simps vs_all_heap_simps valid_release_q_def pred_neg_def
-                         is_blocked_on_reply_def)
+   apply (frule invs_valid_global_refs)
+   apply (frule idle_sc_no_ex_cap; fastforce?)
+   apply (fastforce simp: obj_at_kh_kheap_simps vs_all_heap_simps valid_release_q_def pred_neg_def
+                          is_blocked_on_reply_def)
+  apply (frule invs_valid_global_refs)
+  apply (frule idle_sc_no_ex_cap; fastforce?)
   done
 
 lemma cancel_ipc_heap_refs_inv_sc_tcbs[wp]:
   "cancel_ipc tptr \<lbrace>\<lambda>s. heap_refs_inv (sc_tcbs_of s) (tcb_scps_of s)\<rbrace>"
   by (wpsimp simp: heap_refs_inv_def)
 
+lemma ex_nonz_cap_to_tcb_sched_context:
+  "\<lbrakk>bound_sc_tcb_at ((=) (Some sc_ptr)) thread s; invs s; tcb_at thread s; ex_nonz_cap_to thread s\<rbrakk>
+   \<Longrightarrow> ex_nonz_cap_to sc_ptr s"
+   apply (clarsimp simp: obj_at_def is_tcb_def)
+   apply (rename_tac ko, case_tac ko; clarsimp)
+   apply (rename_tac tcb)
+   apply (prop_tac "valid_tcb thread tcb s")
+    apply (frule invs_valid_objs)
+    apply (fastforce simp: valid_objs_def valid_obj_def)
+   apply (prop_tac "sc_at sc_ptr s")
+    apply (clarsimp simp: pred_tcb_at_def obj_at_def valid_tcb_def valid_bound_obj_def
+                   split: option.splits)
+   apply (clarsimp simp: live_def is_sc_obj_def obj_at_def)
+   apply (rule if_live_then_nonz_capD2; fastforce?)
+   apply (clarsimp simp: live_def live_sc_def pred_tcb_at_def obj_at_def)
+   apply (rename_tac ko n, case_tac ko; clarsimp)
+   apply (clarsimp simp: live_def live_sc_def pred_tcb_at_def obj_at_def)
+   apply (frule invs_sym_refs)
+   apply (elim disjE)
+    apply (frule invs_sym_refs)
+    apply (frule_tac tp=thread in sym_ref_tcb_sc; fastforce?)
+     apply (erule sym)
+    apply fastforce
+   apply (frule invs_valid_idle)
+   apply (clarsimp simp: valid_idle_def pred_tcb_at_def obj_at_def)
+   apply (prop_tac "ex_nonz_cap_to idle_thread_ptr s")
+    apply (rule if_live_then_nonz_capD2; fastforce?)
+    apply (clarsimp simp: live_def)
+    apply (prop_tac "thread \<noteq> idle_thread_ptr")
+     apply (frule invs_valid_global_refs)
+     apply (frule idle_no_ex_cap; fastforce)
+    apply (frule invs_sym_refs)
+    apply (frule_tac tp=thread in sym_ref_tcb_sc)
+      apply fastforce
+     apply (erule sym)
+    apply fastforce
+   apply (frule invs_valid_global_refs)
+   apply (frule idle_no_ex_cap)
+   apply fastforce
+  apply fastforce
+  done
+
 lemma restart_cur_sc_not_in_release_q:
   "\<lbrace>\<lambda>s. sc_not_in_release_q (cur_sc s) s
         \<and> heap_refs_inv (sc_tcbs_of s) (tcb_scps_of s)
         \<and> current_time_bounded 0 s
         \<and> (cur_sc_active s \<longrightarrow> cur_sc_offset_ready (consumed_time s) s
-                               \<and> cur_sc_offset_sufficient (consumed_time s) s)\<rbrace>
+                               \<and> cur_sc_offset_sufficient (consumed_time s) s)
+        \<and> ex_nonz_cap_to thread s
+        \<and> tcb_at thread s
+        \<and> invs s\<rbrace>
    restart thread
    \<lbrace>\<lambda>_ s. sc_not_in_release_q (cur_sc s) s\<rbrace>"
-  unfolding restart_def test_possible_switch_to_def if_cond_refill_unblock_check_def
-  apply (rule hoare_seq_ext_skip, solves \<open>wpsimp\<close>)+
-  apply (rename_tac sc_opt)
-  apply (clarsimp simp: when_def)
-  apply (intro conjI impI; (solves \<open>wpsimp\<close>)?)
-  apply (rule hoare_seq_ext_skip, solves \<open>wpsimp simp: heap_refs_inv_def\<close>)+
-  apply (case_tac sc_opt; simp)
+  apply (clarsimp simp: restart_def test_possible_switch_to_def if_cond_refill_unblock_check_def)
+  apply (rule hoare_seq_ext_skip, solves \<open>wpsimp simp: heap_refs_inv_def\<close>)
+  apply (rule hoare_seq_ext[OF _ gsc_sp])
+  apply (rule hoare_when_cases, simp)
+  apply (rule_tac R1="\<lambda>s. \<forall>sc_ptr. sc_opt = Some sc_ptr \<longrightarrow> sc_ptr \<noteq> idle_sc_ptr"
+               in hoare_pre_add[THEN iffD2, simplified pred_conj_def])
+   apply (intro conjI impI allI)
+   apply (rename_tac sc_ptr)
+   apply (rule_tac scp=sc_ptr in ex_nonz_cap_to_not_idle_sc_ptr)
+    apply fastforce
+   apply (fastforce intro: ex_nonz_cap_to_tcb_sched_context)
+  apply (rule hoare_seq_ext_skip)
+   apply (wpsimp wp: cancel_ipc_cap_to)
+  apply (rule_tac B="\<lambda>_ s. bound_sc_tcb_at ((=) sc_opt) thread s
+                           \<and> sc_not_in_release_q (cur_sc s) s
+                           \<and> heap_refs_inv (sc_tcbs_of s) (tcb_scps_of s)
+                           \<and> current_time_bounded 0 s
+                           \<and> (cur_sc_active s
+                              \<longrightarrow> cur_sc_offset_ready (consumed_time s) s
+                                  \<and> cur_sc_offset_sufficient (consumed_time s) s)
+                           \<and> ex_nonz_cap_to thread s \<and> tcb_at thread s
+                           \<and> (\<forall>sc_ptr. sc_opt = Some sc_ptr \<longrightarrow> sc_ptr \<noteq> idle_sc_ptr)"
+               in hoare_seq_ext[rotated])
    apply wpsimp
-  apply (rename_tac sc_ptr)
-  apply (clarsimp simp: maybeM_def bind_assoc)
-  apply (rule hoare_seq_ext[OF _ get_sched_context_sp])
-  apply (rule hoare_seq_ext[OF _ gets_sp])
-  apply (rename_tac sc cur_scp)
-  apply (rule_tac P="K (cur_scp = sc_ptr)" in hoare_pre_tautI; simp add: pred_neg_def split del: if_split)
-   apply (rule hoare_gen_asm', clarsimp)
-   apply (wpsimp wp: sched_context_resume_cur_sc_not_in_release_q)
-   apply (clarsimp simp: heap_refs_inv_def)
-  using strengthen_cur_sc_offset_ready strengthen_cur_sc_offset_sufficient apply blast
-  apply (rule hoare_gen_asm')
-  apply (rule_tac Q="\<lambda>_ s. cur_sc s \<noteq> sc_ptr \<and> sc_not_in_release_q (cur_sc s) s"
-         in hoare_strengthen_post)
-   apply (wpsimp wp: sched_context_resume_cur_sc_not_in_release_q)
-     apply (rule_tac Q="\<lambda>_ s. cur_sc s \<noteq> sc_ptr \<and> sc_not_in_release_q (cur_sc s) s
-                            \<and> heap_refs_retract (sc_tcbs_of s) (tcb_scps_of s)"
-            in hoare_strengthen_post)
-      apply wpsimp
-     apply clarsimp
-    apply wpsimp
-   apply (clarsimp simp: heap_refs_inv_def)
-  apply simp
+  apply (rule hoare_seq_ext_skip)
+   apply wpsimp
+   apply (clarsimp simp: pred_tcb_at_def obj_at_def)
+  apply (wpsimp wp: sched_context_resume_cur_sc_not_in_release_q)
+  apply (intro conjI impI)
+    apply (rename_tac sc_opt)
+    apply (clarsimp simp: when_def)
+    apply (rule strengthen_cur_sc_offset_ready)
+      apply fastforce
+     apply fastforce
+    apply fastforce
+   apply (rule strengthen_cur_sc_offset_sufficient, fastforce+)
+  apply (clarsimp simp: heap_refs_inv_def)
   done
 
 crunches restart
@@ -23479,7 +23769,8 @@ lemma restart_cur_sc_in_release_q_imp_zero_consumed[wp]:
   "\<lbrace>\<lambda>s. cur_sc_in_release_q_imp_zero_consumed s
         \<and> heap_refs_inv (sc_tcbs_of s) (tcb_scps_of s)
         \<and> cur_sc_more_than_ready s
-        \<and> current_time_bounded 0 s\<rbrace>
+        \<and> current_time_bounded 0 s
+        \<and> invs s \<and> ex_nonz_cap_to thread s \<and> tcb_at thread s\<rbrace>
    restart thread
    \<lbrace>\<lambda>_. cur_sc_in_release_q_imp_zero_consumed\<rbrace>"
   unfolding cur_sc_in_release_q_imp_zero_consumed_def
@@ -24055,6 +24346,23 @@ lemma install_tcb_cap_release_q_not_blocked_on_reply[wp]:
   apply (wpsimp wp: check_cap_inv)
   done
 
+crunches sched_context_yield_to, sched_context_bind_tcb,
+         cancel_badged_sends, restart, maybe_sched_context_unbind_tcb, maybe_sched_context_bind_tcb,
+         sched_context_bind_tcb, bind_notification, send_signal
+  for cur_sc[wp]: "\<lambda>s. P (cur_sc s)"
+  (wp: crunch_wps check_cap_inv filterM_preserved simp: crunch_simps)
+
+crunches install_tcb_cap, install_tcb_frame_cap, do_reply_transfer, invoke_irq_handler, awaken,
+         check_domain_time, if_cond_refill_unblock_check, activate_thread, handle_fault, handle_recv,
+         handle_yield, handle_interrupt, preemption_path
+  for cur_sc[wp]: "\<lambda>s :: det_state. P (cur_sc s)"
+  (wp: crunch_wps check_cap_inv  preemption_point_inv hoare_vcg_all_lift simp: crunch_simps)
+
+crunches perform_invocation
+  for cur_sc[wp]: "\<lambda>s :: det_state. P (cur_sc s)"
+  (wp: crunch_wps preemption_point_inv check_cap_inv filterM_preserved cap_revoke_preservation
+   simp: crunch_simps)
+
 lemma invoke_tcb_cur_sc_in_release_q_imp_zero_consumed[wp]:
   "\<lbrace>\<lambda>s. cur_sc_in_release_q_imp_zero_consumed s
         \<and> cur_sc_in_release_q_imp_zero_consumed_pred s
@@ -24064,7 +24372,8 @@ lemma invoke_tcb_cur_sc_in_release_q_imp_zero_consumed[wp]:
         \<and> valid_sched s \<and> valid_machine_time s
         \<and> tcb_inv_wf iv s
         \<and> (cur_sc_active s \<longrightarrow> cur_sc_offset_ready (consumed_time s) s)
-        \<and> (cur_sc_active s \<longrightarrow> cur_sc_offset_sufficient (consumed_time s) s)\<rbrace>
+        \<and> (cur_sc_active s \<longrightarrow> cur_sc_offset_sufficient (consumed_time s) s)
+        \<and> cur_sc s \<noteq> idle_sc_ptr\<rbrace>
    invoke_tcb iv
    \<lbrace>\<lambda>_ s :: det_state. cur_sc_in_release_q_imp_zero_consumed s\<rbrace>, -"
   apply (cases iv; clarsimp?, (solves \<open>wpsimp\<close>)?)
@@ -24073,20 +24382,28 @@ lemma invoke_tcb_cur_sc_in_release_q_imp_zero_consumed[wp]:
        apply (fastforce simp: current_time_bounded_strengthen)
 
       \<comment> \<open>iv = CopyRegisters\<close>
+      apply (rename_tac dest src suspend_source resume_target transfer_frame transfer_integer transfer_arch)
       apply (clarsimp simp: validE_R_def)
       apply (rule_tac B="\<lambda>_ s. cur_sc_in_release_q_imp_zero_consumed s
                                \<and> heap_refs_inv (sc_tcbs_of s) (tcb_scps_of s)
                                \<and> cur_sc_more_than_ready s
-                               \<and> current_time_bounded 5 s"
+                               \<and> current_time_bounded 5 s \<and> invs s \<and> cur_sc s \<noteq> idle_sc_ptr
+                               \<and> ex_nonz_cap_to dest s \<and> tcb_at dest s"
                    in hoare_seq_ext[rotated])
-      apply wpsimp
-     apply (rule_tac B="\<lambda>_ s. cur_sc_in_release_q_imp_zero_consumed s" in hoare_seq_ext[rotated])
-      apply wpsimp
+       apply (wpsimp wp : suspend_invs)
+       apply (frule invs_valid_global_refs)
+       apply (frule idle_no_ex_cap)
+        apply fastforce
+       apply (frule invs_valid_idle)
+       apply (frule idle_thread_idle_thread_ptr)
+       apply fastforce
+      apply (rule_tac B="\<lambda>_ s. cur_sc_in_release_q_imp_zero_consumed s" in hoare_seq_ext[rotated])
+       apply wpsimp
        apply (fastforce simp: current_time_bounded_strengthen)
 
-     apply (rule hoare_seq_ext_skip, wpsimp wp: mapM_x_wp[where S="set frame_registers"])
-     apply (rule hoare_seq_ext_skip, wpsimp wp: mapM_x_wp[where S="set gpRegisters"])
-     apply wpsimp
+      apply (rule hoare_seq_ext_skip, wpsimp wp: mapM_x_wp[where S="set frame_registers"])
+      apply (rule hoare_seq_ext_skip, wpsimp wp: mapM_x_wp[where S="set gpRegisters"])
+      apply wpsimp
 
      \<comment> \<open>iv = Resume\<close>
      apply (find_goal \<open>match premises in "_ = Resume _" \<Rightarrow> \<open>-\<close>\<close>)
@@ -24118,7 +24435,8 @@ lemma invoke_tcb_cur_sc_in_release_q_imp_zero_consumed[wp]:
                          \<and> (case sc of None \<Rightarrow> \<lambda>_. True
                                      | Some None \<Rightarrow> \<lambda>s. True
                                      | Some (Some scptr) \<Rightarrow> (bound_sc_tcb_at ((=) None) target)
-                                                             and sc_tcb_sc_at ((=) None) scptr) s"
+                                                             and sc_tcb_sc_at ((=) None) scptr) s
+                         \<and> cur_sc s \<noteq> idle_sc_ptr"
                in hoare_weaken_preE[rotated])
    apply (simp add: valid_sched_def)
    apply (clarsimp split: option.splits)
@@ -24136,16 +24454,22 @@ lemma invoke_tcb_cur_sc_in_release_q_imp_zero_consumed[wp]:
                            \<and> (case sc of None \<Rightarrow> \<lambda>_. True
                                        | Some None \<Rightarrow> \<lambda>s. True
                                        | Some (Some scptr) \<Rightarrow> (bound_sc_tcb_at ((=) None) target)
-                                                               and sc_tcb_sc_at ((=) None) scptr) s"
+                                                               and sc_tcb_sc_at ((=) None) scptr
+                                                               and K (scptr \<noteq> idle_sc_ptr)) s
+                           \<and> cur_sc s \<noteq> idle_sc_ptr"
                in hoare_vcg_seqE[rotated])
    apply (rule hoare_weaken_preE)
     apply (subst validE_R_def[symmetric])
     apply (rule hoare_vcg_conj_lift_R)
      apply wpsimp
-    apply (wpsimp wp: hoare_case_option_wp install_tcb_cap_sc_tcb_sc_at)
+    apply (wpsimp wp: hoare_case_option_wp install_tcb_cap_sc_tcb_sc_at)+
    apply (clarsimp split: option.splits)
-
+   apply (intro conjI impI)
+    apply (clarsimp simp: pred_tcb_at_def obj_at_def is_tcb_def)
+   apply (frule invs_valid_idle)
+   apply (clarsimp simp: valid_idle_def pred_tcb_at_def obj_at_def sc_at_pred_n_def)
   apply (rule hoare_seq_ext_skipE, wpsimp wp: thread_set_wp simp: set_mcpriority_def)
+   apply (clarsimp split: option.splits)
    apply (fastforce simp: pred_tcb_at_def sc_at_pred_n_def obj_at_def get_tcb_def
                    split: option.splits)
   apply (rule hoare_seq_ext_skipE, wpsimp wp: hoare_case_option_wp)
@@ -24169,8 +24493,7 @@ lemma invoke_tcb_cur_sc_in_release_q_imp_zero_consumed[wp]:
   apply (rule hoare_seq_ext[OF _ gsc_sp])
   apply (rule hoare_when_cases; (solves \<open>wpsimp\<close>)?)
    apply wpsimp
-   apply (fastforce simp: pred_tcb_at_def sc_at_pred_n_def obj_at_def vs_all_heap_simps pred_neg_def
-                          is_blocked_on_reply_def current_time_bounded_strengthen)
+   apply (fastforce simp: cur_sc_in_release_q_imp_zero_consumed_def)
   apply wpsimp
   apply (fastforce simp: pred_tcb_at_def sc_at_pred_n_def obj_at_def vs_all_heap_simps pred_neg_def
                          is_blocked_on_reply_def current_time_bounded_strengthen
@@ -24217,7 +24540,7 @@ lemma perform_invocation_cur_sc_in_release_q_imp_zero_consumed:
   "\<lbrace>\<lambda>s. cur_sc_in_release_q_imp_zero_consumed s
         \<and> cur_sc_more_than_ready s
         \<and> valid_sched s \<and> valid_machine_time s
-        \<and> invs s
+        \<and> invs s \<and> cur_sc_tcb_are_bound s
         \<and> current_time_bounded 5 s
         \<and> ct_not_in_release_q s
         \<and> ct_active s
@@ -24238,16 +24561,20 @@ lemma perform_invocation_cur_sc_in_release_q_imp_zero_consumed:
         apply (wpsimp wp: send_signal_cur_sc_in_release_q_imp_zero_consumed)
         apply (fastforce simp: current_time_bounded_strengthen)
        apply (wpsimp wp: do_reply_transfer_cur_sc_in_release_q_imp_zero_consumed)
-       apply (fastforce intro: current_time_bounded_strengthen)
+       apply (intro conjI; fastforce?)
+        apply (clarsimp simp: current_time_bounded_def)
+       apply (rule cur_sc_not_idle_sc_ptr; fastforce)
       apply wpsimp
-      apply (fastforce dest!: invs_strengthen_cur_sc_tcb_only_sym_bound
-                              cur_sc_tcb_only_sym_bound_cur_sc_not_in_release_q
-                      intro!: valid_release_q_imp_not_blocked_on_reply
-                              valid_release_q_imp_bound_to_sc)
+      apply (intro conjI)
+         apply (fastforce dest!: invs_strengthen_cur_sc_tcb_only_sym_bound
+                                 cur_sc_tcb_only_sym_bound_cur_sc_not_in_release_q)
+        apply (fastforce intro!: valid_release_q_imp_not_blocked_on_reply)
+       apply (fastforce intro!: valid_release_q_imp_bound_to_sc)
+      apply (rule cur_sc_not_idle_sc_ptr; fastforce)
      apply wpsimp
      apply (fastforce elim: current_time_bounded_strengthen)
     apply wpsimp
-    apply (fastforce elim: current_time_bounded_strengthen)
+    apply (fastforce simp: current_time_bounded_strengthen)
    apply (clarsimp simp: validE_R_def)
    apply (rule_tac P'="?P"
                and Q'="\<lambda>_. cur_sc_in_release_q_imp_zero_consumed_pred"
@@ -24289,7 +24616,7 @@ lemma handle_invocation_cur_sc_in_release_q_imp_zero_consumed[wp]:
   "\<lbrace>\<lambda>s. cur_sc_in_release_q_imp_zero_consumed s
     \<and> cur_sc_more_than_ready s
     \<and> valid_sched s \<and> valid_machine_time s
-    \<and> invs s
+    \<and> invs s \<and> cur_sc_tcb_are_bound s
     \<and> current_time_bounded 5 s
     \<and> ct_not_in_release_q s
     \<and> cur_sc_active s
@@ -24304,15 +24631,14 @@ lemma handle_invocation_cur_sc_in_release_q_imp_zero_consumed[wp]:
   apply (wpsimp wp: syscall_valid)
          apply (wpsimp wp: hoare_drop_imp, clarsimp)
         apply (wpsimp wp: perform_invocation_cur_sc_in_release_q_imp_zero_consumed, clarsimp)
-       apply (wpsimp wp: set_thread_state_runnable_valid_sched set_thread_state_ct_in_state
-              , clarsimp simp: runnable_eq_active)
+       apply (wpsimp wp: set_thread_state_runnable_valid_sched set_thread_state_ct_in_state)
       apply wpsimp
      apply (wpsimp simp: cap_cap_slot_fold)
     apply wpsimp
    apply wpsimp
-  apply (auto dest!: ct_active_not_receive_blocked_helper
-              split: if_split
-               simp: ct_in_state_def2[symmetric] current_time_bounded_strengthen)
+  apply (fastforce simp: ct_in_state_def pred_tcb_at_def obj_at_def runnable_eq_active
+                         vs_all_heap_simps receive_blocked_def is_tcb_def
+                  split: if_splits)
   done
 
 lemma charge_budget_consumed_time_equals_zero[wp]:
@@ -24345,9 +24671,41 @@ lemma handle_yield_cur_sc_in_release_q_imp_zero_consumed[wp]:
   unfolding handle_yield_def
   by wpsimp
 
-crunches complete_signal, do_nbrecv_failed_transfer, lookup_reply, schedule_tcb, test_reschedule
+crunches do_nbrecv_failed_transfer, lookup_reply, schedule_tcb, test_reschedule
   for cur_sc_in_release_q_imp_zero_consumed[wp]: cur_sc_in_release_q_imp_zero_consumed
   (wp: hoare_vcg_all_lift crunch_wps)
+
+lemma complete_signal_cur_sc_in_release_q_imp_zero_consumed:
+  "\<lbrace>cur_sc_in_release_q_imp_zero_consumed and cur_sc_more_than_ready and not_in_release_q tptr
+    and current_time_bounded 0 and ex_nonz_cap_to tptr and tcb_at tptr and invs\<rbrace>
+   complete_signal ntfnptr tptr
+   \<lbrace>\<lambda>_. cur_sc_in_release_q_imp_zero_consumed :: det_state \<Rightarrow> _\<rbrace>"
+  apply (simp add: complete_signal_def)
+  apply (rule hoare_seq_ext[OF _ get_simple_ko_sp])
+  apply (case_tac "ntfn_obj ntfn"; simp)
+  apply (rule hoare_seq_ext_skip)
+   apply (clarsimp simp: pred_conj_def)
+   apply (intro hoare_vcg_conj_lift_pre_fix; (solves wpsimp)?)
+   apply (wpsimp simp: as_user_def
+                   wp: set_object_wp get_object_wp)
+   apply (clarsimp simp: obj_at_def get_tcb_def)
+  apply (wpsimp simp: get_tcb_obj_ref_def wp: thread_get_wp)
+     apply (rule hoare_strengthen_post[where Q="\<lambda>_. cur_sc_in_release_q_imp_zero_consumed and invs
+                                                    and tcb_at tptr"])
+      apply (wpsimp wp: maybe_donate_sc_cur_sc_in_release_q_imp_zero_consumed abs_typ_at_lifts)
+     apply (clarsimp simp: obj_at_def)
+    apply (wpsimp wp: set_ntfn_minor_invs simp: as_user_def set_object_def get_object_def)+
+  apply (intro conjI impI allI)
+    apply (clarsimp simp: obj_at_def is_tcb)
+   apply (fastforce simp: invs_def valid_state_def valid_pspace_def valid_bound_obj_def
+                          valid_obj_def valid_ntfn_def is_tcb obj_at_def is_sc_obj_def
+                   elim!: valid_objsE
+                   split: option.splits)
+  apply (fastforce simp: invs_def valid_state_def valid_pspace_def live_def live_ntfn_def
+                         tcb_cap_cases_def is_tcb obj_at_def
+                 intro!: ex_cap_to_after_update
+                  elim!: if_live_then_nonz_capD)
+  done
 
 lemma set_tcb_sc_Some_cur_sc_in_release_q_imp_zero_consumed[wp]:
   "\<lbrace>cur_sc_in_release_q_imp_zero_consumed and not_in_release_q tptr\<rbrace>
@@ -24459,7 +24817,8 @@ lemma receive_ipc_cur_sc_in_release_q_imp_zero_consumed[wp]:
     and scheduler_act_not thread and not_queued thread and not_in_release_q thread
     and (\<lambda>s. heap_refs_inv (sc_tcbs_of s) (tcb_scps_of s))
     and cur_sc_more_than_ready and current_time_bounded 2
-    and (\<lambda>s. thread = cur_thread s)\<rbrace>
+    and (\<lambda>s. thread = cur_thread s) and invs
+    and st_tcb_at active thread\<rbrace>
    receive_ipc thread cap is_blocking reply_cap
    \<lbrace>\<lambda>_. cur_sc_in_release_q_imp_zero_consumed :: det_state \<Rightarrow> _\<rbrace>"
   supply if_split[split del]
@@ -24474,14 +24833,35 @@ lemma receive_ipc_cur_sc_in_release_q_imp_zero_consumed[wp]:
   apply (rule hoare_seq_ext[OF _ gbn_sp])
   apply (case_tac ep; simp; (solves \<open>wpsimp wp: get_simple_ko_wp
                                           simp: current_time_bounded_def heap_refs_inv_def\<close>)?)
-  apply (rename_tac qs)
+
+    apply (find_goal \<open>match premises in "_ = IdleEP" \<Rightarrow> \<open>-\<close>\<close>)
+    apply (wpsimp wp: get_simple_ko_wp complete_signal_cur_sc_in_release_q_imp_zero_consumed)
+    apply (fastforce dest: invs_cur
+                    intro: runnable_nonz_cap_to
+                     simp: current_time_bounded_def runnable_eq_active cur_tcb_def)
+
+   apply (find_goal \<open>match premises in "_ = RecvEP _" \<Rightarrow> \<open>-\<close>\<close>)
+   apply (wpsimp wp: get_simple_ko_wp thread_get_inv hoare_drop_imps
+                     complete_signal_cur_sc_in_release_q_imp_zero_consumed)
+   apply (fastforce intro: runnable_nonz_cap_to simp: runnable_eq_active current_time_bounded_def)
+
+  apply (rule hoare_seq_ext_skip, wpsimp)
+   apply (clarsimp simp: pred_tcb_at_def obj_at_def)
+  apply (rule hoare_if)
+   apply (wpsimp wp: refill_unblock_check_valid_release_q
+                     complete_signal_cur_sc_in_release_q_imp_zero_consumed)
+    apply (fastforce dest: invs_cur
+                    intro: runnable_nonz_cap_to
+                     simp: current_time_bounded_def runnable_eq_active cur_tcb_def)
+  apply (rename_tac qs ntfn)
   apply (wpsimp wp: thread_get_wp')
               apply (rule_tac Q="\<lambda>_ s. cur_sc_in_release_q_imp_zero_consumed s
                                       \<and> valid_release_q s \<and> not_in_release_q (hd qs) s
                                       \<and> heap_refs_inv (sc_tcbs_of s) (tcb_scps_of s)"
                     in hoare_post_imp)
               apply clarsimp
-             apply (wpsimp wp: refill_unblock_check_valid_release_q)
+             apply (wpsimp wp: refill_unblock_check_valid_release_q
+                               complete_signal_cur_sc_in_release_q_imp_zero_consumed)
             apply (wpsimp+)[3]
           apply (wpsimp wp: get_tcb_obj_ref_wp)
          (* do_ipc_transfer *)
@@ -24512,26 +24892,41 @@ lemma receive_ipc_cur_sc_in_release_q_imp_zero_consumed[wp]:
     apply (rule hoare_drop_imp)
     apply (wpsimp wp : hoare_vcg_imp_lift')
    apply wpsimp
-   apply (wpsimp wp: get_simple_ko_wp)
-  apply (clarsimp)
-  apply (intro conjI; clarsimp simp: valid_sched_def)
-  by (fastforce dest: valid_release_q_ipc_queued_thread_state_not_in_release_q
-                simp: ipc_queued_thread_state_def2 not_in_release_q_def heap_refs_inv_def
-                      current_time_bounded_def
-                elim: pred_tcb_weakenE split: if_split)+
+  apply (clarsimp cong: conj_cong
+                 split: if_splits)
+  apply (frule valid_sched_valid_release_q)
+  apply (fastforce simp: pred_tcb_at_def obj_at_def is_blocked_on_send_def in_release_q_def
+                         valid_release_q_def vs_all_heap_simps )
+  done
 
+crunches as_user
+  for valid_ntfn[wp]: "valid_ntfn ntfn"
 
 lemma receive_signal_cur_sc_in_release_q_imp_zero_consumed[wp]:
   "\<lbrace>\<lambda>s. cur_sc_in_release_q_imp_zero_consumed s
         \<and> heap_refs_retract (sc_tcbs_of s) (tcb_scps_of s)
         \<and> cur_sc_more_than_ready s
         \<and> not_in_release_q thread s
-        \<and> current_time_bounded 0 s\<rbrace>
+        \<and> current_time_bounded 0 s \<and> invs s \<and> thread = cur_thread s \<and> st_tcb_at runnable thread s\<rbrace>
    receive_signal thread cap is_blocking
    \<lbrace>\<lambda>_. cur_sc_in_release_q_imp_zero_consumed :: det_state \<Rightarrow> _\<rbrace>"
   unfolding receive_signal_def
   apply (wpsimp wp: hoare_drop_imp hoare_vcg_all_lift)
-       apply (wpsimp wp: maybe_donate_sc_cur_sc_in_release_q_imp_zero_consumed get_simple_ko_wp)+
+       apply (wpsimp wp: maybe_donate_sc_cur_sc_in_release_q_imp_zero_consumed get_simple_ko_wp
+                         set_ntfn_minor_invs as_user_obj_at_trivial hoare_vcg_imp_lift')+
+  apply (intro conjI impI)
+     apply (fastforce intro: runnable_nonz_cap_to
+                       simp: runnable_eq_active)
+    apply (clarsimp simp: obj_at_def)
+   apply (clarsimp simp: obj_at_def)
+   apply (frule invs_valid_objs)
+   apply (frule valid_objs_valid_ntfn)
+    apply fastforce
+   apply (clarsimp simp: valid_ntfn_def valid_bound_obj_def)
+  apply (rule if_live_then_nonz_capD2)
+    apply fastforce
+   apply (fastforce simp: obj_at_def)
+  apply (clarsimp simp: live_def live_ntfn_def)
   done
 
 lemma handle_recv_cur_sc_in_release_q_imp_zero_consumed[wp]:
@@ -24543,7 +24938,7 @@ lemma handle_recv_cur_sc_in_release_q_imp_zero_consumed[wp]:
         \<and> current_time_bounded 2 s
         \<and> ct_not_in_release_q s
         \<and> scheduler_act_sane s
-        \<and> ct_not_queued s\<rbrace>
+        \<and> ct_not_queued s \<and> invs s\<rbrace>
    handle_recv is_blocking can_reply
    \<lbrace>\<lambda>_. cur_sc_in_release_q_imp_zero_consumed :: det_state \<Rightarrow> _\<rbrace>"
   unfolding handle_recv_def Let_def
@@ -24555,9 +24950,10 @@ lemma handle_recv_cur_sc_in_release_q_imp_zero_consumed[wp]:
                                \<and> current_time_bounded 2 s
                                \<and> not_in_release_q thread s \<and> scheduler_act_not thread s \<and> not_queued thread s
                                \<and> \<not> pred_map receive_blocked (tcb_sts_of s) thread
-                               \<and> heap_refs_inj_at thread (tcb_scps_of s)"
+                               \<and> heap_refs_inj_at thread (tcb_scps_of s) \<and> invs s \<and> ct_active s"
                in hoare_post_imp_R[rotated])
-      apply (clarsimp simp: current_time_bounded_def valid_sched_valid_release_q)
+      apply (clarsimp simp: current_time_bounded_def valid_sched_valid_release_q ct_in_state_def
+                            runnable_eq_active)
      apply wpsimp+
   apply (fastforce dest: valid_sched_valid_release_q ct_active_not_receive_blocked_helper
                          heap_refs_injD sym_refs_inj_tcb_scps invs_sym_refs)
@@ -25178,7 +25574,7 @@ lemma refill_budget_check_round_robin_ct_ready_if_schedulable[wp]:
   "\<lbrace>\<lambda>s. bound_sc_tcb_at (\<lambda>a. a = Some (cur_sc s)) (cur_thread s) s
         \<and> current_time_bounded 0 s
         \<and> cur_sc_offset_ready consumed s
-        \<and> cur_sc_offset_sufficient consumed s\<rbrace>
+        \<and> cur_sc_offset_sufficient consumed s \<and> cur_sc s \<noteq> idle_sc_ptr\<rbrace>
    refill_budget_check_round_robin consumed
    \<lbrace>\<lambda>_. ct_ready_if_schedulable\<rbrace>"
   unfolding ct_ready_if_schedulable_def
@@ -25193,7 +25589,7 @@ lemma refill_budget_check_ct_ready_if_schedulable[wp]:
   "\<lbrace>\<lambda>s. valid_refills (cur_sc s) s \<and> bound_sc_tcb_at (\<lambda>a. a = Some (cur_sc s)) (cur_thread s) s
         \<and> current_time_bounded 5 s
         \<and> cur_sc_offset_ready consumed s
-        \<and> cur_sc_offset_sufficient consumed s\<rbrace>
+        \<and> cur_sc_offset_sufficient consumed s \<and> cur_sc s \<noteq> idle_sc_ptr\<rbrace>
    refill_budget_check consumed
    \<lbrace>\<lambda>_. ct_ready_if_schedulable\<rbrace>"
   unfolding ct_ready_if_schedulable_def
@@ -25232,7 +25628,7 @@ lemma invoke_sched_control_configure_flags_ct_ready_if_schedulable[wp]:
     and schact_is_rct
     and invs
     and current_time_bounded 5
-    and valid_sched_control_inv iv\<rbrace>
+    and valid_sched_control_inv iv and (\<lambda>s. cur_sc s \<noteq> idle_sc_ptr)\<rbrace>
    invoke_sched_control_configure_flags iv
    \<lbrace>\<lambda>_. ct_ready_if_schedulable\<rbrace>"
   supply if_split [split del]
@@ -25249,7 +25645,7 @@ lemma invoke_sched_control_configure_flags_ct_ready_if_schedulable[wp]:
                               \<and> MIN_BUDGET \<le> budget
                               \<and> (sc_active sc \<longrightarrow> is_active_sc sc_ptr s)
                               \<and> (sc_tcb_sc_at ((=) (sc_tcb sc)) sc_ptr s)
-                              \<and> invs s"
+                              \<and> invs s \<and> cur_sc s \<noteq> idle_sc_ptr"
             in hoare_post_imp)
       apply (clarsimp simp: current_time_bounded_def)
       apply (subgoal_tac "y = cur_thread s")
@@ -25268,13 +25664,12 @@ lemma invoke_sched_control_configure_flags_ct_ready_if_schedulable[wp]:
                              \<and> sc_tcb_sc_at ((=) (sc_tcb sc)) sc_ptr s
                              \<and> cur_sc_offset_ready (consumed_time s) s
                              \<and> cur_sc_offset_sufficient (consumed_time s) s
-                             \<and> MIN_BUDGET \<le> budget"
+                             \<and> MIN_BUDGET \<le> budget \<and> cur_sc s \<noteq> idle_sc_ptr"
            in hoare_post_imp)
     apply (subgoal_tac "budget_ready (cur_thread s) s")
      apply (fastforce simp: ct_ready_if_schedulable_def current_time_bounded_def split: if_split)
     apply (clarsimp simp: tcb_at_kh_simps pred_map_eq_normalise)
-    apply (erule (1) cur_sc_tcb_bound_ready)
-    apply simp
+    apply (rule cur_sc_tcb_bound_ready; fastforce)
    apply (wpsimp wp: update_sc_badge_invs' update_sc_sporadic_invs' simp: sc_at_kh_simps)+
   apply (subgoal_tac "cur_sc_chargeable s", simp)
    apply (intro conjI)
@@ -25333,7 +25728,7 @@ lemma perform_unsafe_invocation_ct_ready_if_schedulable:
     and current_time_bounded 5
     and cur_sc_active
     and (\<lambda>s. cur_sc_offset_ready (consumed_time s) s \<and> cur_sc_offset_sufficient (consumed_time s) s)
-    and (\<lambda>s. bound_sc_tcb_at bound (cur_thread s) s)\<rbrace>
+    and (\<lambda>s. bound_sc_tcb_at bound (cur_thread s) s) and (\<lambda>s. cur_sc s \<noteq> idle_sc_ptr)\<rbrace>
    perform_invocation block call can_donate i
    \<lbrace>\<lambda>_ s :: det_state. ct_ready_if_schedulable s\<rbrace>"
   apply (cases i; simp)
@@ -25360,7 +25755,7 @@ lemma perform_invocation_ct_ready_if_schedulable[wp]:
     and current_time_bounded 5
     and cur_sc_active
     and (\<lambda>s. cur_sc_offset_ready (consumed_time s) s \<and> cur_sc_offset_sufficient (consumed_time s) s)
-    and (\<lambda>s. bound_sc_tcb_at bound (cur_thread s) s)\<rbrace>
+    and (\<lambda>s. bound_sc_tcb_at bound (cur_thread s) s) and (\<lambda>s. cur_sc s \<noteq> idle_sc_ptr)\<rbrace>
    perform_invocation block call can_donate i
    \<lbrace>\<lambda>_ s :: det_state. ct_ready_if_schedulable s\<rbrace>"
   apply (case_tac "safe_invocation i")
@@ -25398,7 +25793,8 @@ lemma handle_invocation_ct_ready_if_schedulable[wp]:
     and current_time_bounded 5
     and (\<lambda>s. cur_sc_active s \<longrightarrow> cur_sc_offset_ready (consumed_time s) s)
     and (\<lambda>s. cur_sc_offset_sufficient (consumed_time s) s)
-    and ct_released\<rbrace>
+    and ct_released
+    and (\<lambda>s. cur_sc s \<noteq> idle_sc_ptr)\<rbrace>
    handle_invocation calling blocking can_donate first_phase cptr
    \<lbrace>\<lambda>_. ct_ready_if_schedulable :: det_state \<Rightarrow> _\<rbrace>"
   supply if_split [split del]
@@ -25429,7 +25825,7 @@ lemma handle_invocation_ct_ready_if_schedulable[wp]:
                (active_sc_tcb_at (cur_thread s) s \<and> ct_not_in_release_q s) \<and>
                current_time_bounded 5 s \<and>
                cur_sc_offset_ready (consumed_time s) s \<and> cur_sc_offset_sufficient (consumed_time s) s \<and>
-               bound_sc_tcb_at bound (cur_thread s) s \<and> thread = cur_thread s"
+               bound_sc_tcb_at bound (cur_thread s) s \<and> thread = cur_thread s \<and> cur_sc s \<noteq> idle_sc_ptr"
              and E="\<lambda>_. ct_ready_if_schedulable"
              in hoare_post_impErr[rotated])
         apply (clarsimp simp: ct_in_state_def runnable_eq_active)
@@ -25796,11 +26192,12 @@ method he_ctris_two_phase_wp
        | strengthen current_time_bounded_strengthen[where n=1 and k=5, simplified])+)
 
 method he_ctris_two_phase_ff
- = (fastforce intro!: schact_is_rct_ct_released
-                      schact_is_rct_ct_active_sc
-                simp: runnable_eq_active ct_in_state_def in_release_queue_def not_in_release_q_def
-                      schedulable_def2 pred_tcb_at_def obj_at_def
-                elim: invs_cur_sc_chargeableE)
+ = (frule invs_strengthen_cur_sc_tcb_are_bound; fastforce?),
+   fastforce dest: cur_sc_not_idle_sc_ptr'
+           intro!: schact_is_rct_ct_released invs_strengthen_cur_sc_tcb_are_bound
+                   schact_is_rct_ct_active_sc invs_cur_sc_chargeableE
+             simp: runnable_eq_active ct_in_state_def in_release_queue_def not_in_release_q_def
+                   schedulable_def2 pred_tcb_at_def obj_at_def
 
 lemma handle_event_ct_ready_if_schedulable[wp]:
   "\<lbrace>invs
@@ -25838,6 +26235,7 @@ lemma handle_event_ct_ready_if_schedulable[wp]:
      apply he_ctris_handle_recv
     apply he_ctris_handle_recv
     done
+
       apply he_ctris_handle_fault
      apply he_ctris_handle_fault
   subgoal \<comment>\<open>Interrupt\<close>
@@ -25885,15 +26283,15 @@ lemma preemption_path_cur_sc_in_release_q_imp_zero_consumed:
    apply (fastforce simp: schedulable_def2 cur_sc_chargeable_def vs_all_heap_simps
                           current_time_bounded_def)
   apply (intro hoare_vcg_conj_lift_pre_fix; (solves wpsimp)?)
-     apply (wpsimp wp: charge_budget_active_sc_valid_refills)
-     apply (fastforce simp: obj_at_def vs_all_heap_simps
-                      dest: consumed_time_bounded_helper[OF _ current_time_bounded_strengthen])
-    apply (wpsimp wp: charge_budget_valid_release_q)
-    apply (fastforce intro: active_sc_valid_refillsE
-                      simp: obj_at_def vs_all_heap_simps active_sc_def)
-   apply wpsimp
-   apply (clarsimp simp: obj_at_def vs_all_heap_simps cur_sc_more_than_ready_def)
-  apply (wpsimp simp: current_time_bounded_def)
+    apply (wpsimp wp: charge_budget_active_sc_valid_refills)
+    apply (fastforce simp: obj_at_def vs_all_heap_simps refill_ready_no_overflow_def
+                     dest: consumed_time_bounded_helper[OF _ current_time_bounded_strengthen]
+                           valid_sched_active_sc_valid_refills)
+   apply (wpsimp wp: charge_budget_valid_release_q)
+   apply (fastforce intro: active_sc_valid_refillsE
+                     simp: obj_at_def vs_all_heap_simps active_sc_def)
+  apply wpsimp
+  apply (clarsimp simp: current_time_bounded_def)
   done
 
 lemma preemption_path_cur_sc_more_than_ready:
@@ -25935,8 +26333,9 @@ lemma preemption_path_ct_ready_if_schedulable:
    apply (fastforce simp: vs_all_heap_simps schedulable_def2 cur_sc_chargeable_def
                     dest: consumed_time_bounded_helper[OF _ current_time_bounded_strengthen])
   apply (wpsimp wp: charge_budget_ready_if_schedulable)
-  apply (fastforce simp: obj_at_def vs_all_heap_simps
-                   dest: consumed_time_bounded_helper[OF _ current_time_bounded_strengthen])
+  apply (fastforce simp: obj_at_def vs_all_heap_simps refill_ready_no_overflow_def
+                   dest: consumed_time_bounded_helper[OF _ current_time_bounded_strengthen]
+                         valid_sched_active_sc_valid_refills)
   done
 
 lemma preemption_path_valid_sched:
@@ -25971,7 +26370,7 @@ lemma preemption_path_valid_sched:
   apply (wpsimp wp: charge_budget_valid_sched)
   apply (fastforce intro: ct_not_blocked_cur_sc_not_blocked
                           consumed_time_bounded_helper[OF _ current_time_bounded_strengthen]
-                    simp: obj_at_def vs_all_heap_simps)
+                    simp: obj_at_def vs_all_heap_simps refill_ready_no_overflow_def)
   done
 
 lemma preemption_path_invs[wp]:
